Moved byte-aligned decoding components into separate file.

src/BinEncoders/Env/Examples/SimpleDnsOpt.v
@@ -88,16 +88,16 @@ Section DnsPacket.
   Instance cacheAddNat : CacheAdd _ nat :=
     {| addE ce n := (Ifopt (fst ce) as m Then
                                          let n' := (wordToNat m) + n in
-                     if Compare_dec.lt_dec n' (pow2 17)
-                     then Some (natToWord _ n')
-                     else None
-                            Else None, snd ce);
+                                         if Compare_dec.lt_dec n' (pow2 17)
+                                         then Some (natToWord _ n')
+                                         else None
+                                                Else None, snd ce);
        addD cd n := (Ifopt (fst cd) as m Then
                                          let n' := (wordToNat m) + n in
-                     if Compare_dec.lt_dec n' (pow2 17)
-                     then Some (natToWord _ n')
-                     else None
-                            Else None, snd cd) |}.
+                                         if Compare_dec.lt_dec n' (pow2 17)
+                                         then Some (natToWord _ n')
+                                         else None
+                                                Else None, snd cd) |}.
   Proof.
     simpl; intuition eauto; destruct a; destruct a0;
       simpl in *; eauto; try congruence.
@@ -154,10 +154,10 @@ Section DnsPacket.
 
   Lemma cacheAddDNPointer_pf
     : forall (ce : CacheEncode) (cd : CacheDecode) (t : string * pointerT),
-   Equiv ce cd ->
-   add_ptr_OK t ce cd ->
-   Equiv (fst ce, association_list_add (snd ce) (fst t) (snd t))
-     (fst cd, association_list_add (snd cd) (snd t) (fst t)).
+      Equiv ce cd ->
+      add_ptr_OK t ce cd ->
+      Equiv (fst ce, association_list_add (snd ce) (fst t) (snd t))
+            (fst cd, association_list_add (snd cd) (snd t) (fst t)).
   Proof.
     simpl; intuition eauto; simpl in *; subst; eauto.
     unfold add_ptr_OK in *.
@@ -439,7 +439,7 @@ Section DnsPacket.
           peekE (addE env (n * 8)) = Some p'
           /\ pointerT2Nat p' = n + (pointerT2Nat m).
   Proof.
-        simpl; intros; subst.
+    simpl; intros; subst.
     destruct (fst env); simpl in *; try discriminate.
     injections.
     find_if_inside.
@@ -498,9 +498,9 @@ Section DnsPacket.
   Qed.
 
   Lemma addPeekENone :
-      forall env n,
-        peekE env = None
-        -> peekE (addE env n) = None.
+    forall env n,
+      peekE env = None
+      -> peekE (addE env n) = None.
   Proof.
     simpl; intros.
     destruct (fst env); simpl in *; congruence.
@@ -735,47 +735,47 @@ Section DnsPacket.
   Qed.
 
   Lemma cacheIndependent_add_12
-      : forall (p : pointerT) (cd : CacheDecode) (domain : string),
-        GoodCache cd ->
-        getD cd p = Some domain
-        -> forall p' : pointerT,
-            peekD cd = Some p'
-            -> lt (pointerT2Nat p) (pointerT2Nat p').
-    Proof.
-      unfold GoodCache; simpl; intros; intuition eauto.
-      eapply H; eauto.
-    Qed.
+    : forall (p : pointerT) (cd : CacheDecode) (domain : string),
+      GoodCache cd ->
+      getD cd p = Some domain
+      -> forall p' : pointerT,
+          peekD cd = Some p'
+          -> lt (pointerT2Nat p) (pointerT2Nat p').
+  Proof.
+    unfold GoodCache; simpl; intros; intuition eauto.
+    eapply H; eauto.
+  Qed.
 
-    Lemma cacheIndependent_add_13
-      : forall  (env : CacheDecode)
-                (p : pointerT)
-                (domain : string)
-                (H : GoodCache env)
-                (H0 : ValidDomainName domain /\ (String.length domain > 0)%nat)
-                (H1 : getD env p = None)
-                (H2 : forall p' : pointerT, peekD env = Some p' -> lt (pointerT2Nat p) (pointerT2Nat p'))
-                (domain0 : string)
-                (p0 : pointerT)
-                (H3 : getD (addD_G env (domain, p)) p0 = Some domain0)
-                (p' : pointerT),
-        peekD (addD_G env (domain, p)) = Some p'
-        -> lt (pointerT2Nat p0) (pointerT2Nat p').
-    Proof.
-      simpl; intros.
-      destruct (fst env) eqn: ?; simpl in *; try discriminate.
-      find_if_inside; subst.
-      - injections.
-        apply (H2 _ (eq_refl _)).
-      - injections.
-        pose proof (H2 _ (eq_refl _)).
-        unfold GoodCache in *; intuition.
-        eapply H; simpl.
-        eassumption.
-        eassumption.
-        rewrite Heqo; simpl; reflexivity.
-    Qed.
+  Lemma cacheIndependent_add_13
+    : forall  (env : CacheDecode)
+              (p : pointerT)
+              (domain : string)
+              (H : GoodCache env)
+              (H0 : ValidDomainName domain /\ (String.length domain > 0)%nat)
+              (H1 : getD env p = None)
+              (H2 : forall p' : pointerT, peekD env = Some p' -> lt (pointerT2Nat p) (pointerT2Nat p'))
+              (domain0 : string)
+              (p0 : pointerT)
+              (H3 : getD (addD_G env (domain, p)) p0 = Some domain0)
+              (p' : pointerT),
+      peekD (addD_G env (domain, p)) = Some p'
+      -> lt (pointerT2Nat p0) (pointerT2Nat p').
+  Proof.
+    simpl; intros.
+    destruct (fst env) eqn: ?; simpl in *; try discriminate.
+    find_if_inside; subst.
+    - injections.
+      apply (H2 _ (eq_refl _)).
+    - injections.
+      pose proof (H2 _ (eq_refl _)).
+      unfold GoodCache in *; intuition.
+      eapply H; simpl.
+      eassumption.
+      eassumption.
+      rewrite Heqo; simpl; reflexivity.
+  Qed.
 
-    Ltac solve_GoodCache_inv foo :=
+  Ltac solve_GoodCache_inv foo :=
     lazymatch goal with
       |- cache_inv_Property ?Z _ =>
       unify Z GoodCache;
@@ -827,10 +827,10 @@ Section DnsPacket.
   Definition resourceRecord_OK (rr : resourceRecord) :=
     ith
       (icons (B := fun T => T -> Prop) (fun a : DomainName => ValidDomainName a)
-      (icons (B := fun T => T -> Prop) (fun _ : Memory.W => True)
-      (icons (B := fun T => T -> Prop) (fun a : DomainName => ValidDomainName a)
-      (icons (B := fun T => T -> Prop) (fun a : SOA_RDATA =>
-                                          (True /\ ValidDomainName a!"contact_email") /\ ValidDomainName a!"sourcehost") inil))))
+             (icons (B := fun T => T -> Prop) (fun _ : Memory.W => True)
+                    (icons (B := fun T => T -> Prop) (fun a : DomainName => ValidDomainName a)
+                           (icons (B := fun T => T -> Prop) (fun a : SOA_RDATA =>
+                                                               (True /\ ValidDomainName a!"contact_email") /\ ValidDomainName a!"sourcehost") inil))))
       (SumType_index
          (DomainName
             :: (Memory.W : Type)
@@ -858,9 +858,9 @@ Section DnsPacket.
       resourceRecord_OK rr ->
       ith
         (icons (B := fun T => T -> Prop) (fun a : DomainName => ValidDomainName a)
-        (icons (B := fun T => T -> Prop) (fun _ : Memory.W => True)
-        (icons (B := fun T => T -> Prop) (fun a : DomainName => ValidDomainName a)
-        (icons (B := fun T => T -> Prop) (fun a : SOA_RDATA =>
+               (icons (B := fun T => T -> Prop) (fun _ : Memory.W => True)
+                      (icons (B := fun T => T -> Prop) (fun a : DomainName => ValidDomainName a)
+                             (icons (B := fun T => T -> Prop) (fun a : SOA_RDATA =>
                                                                  (True /\ ValidDomainName a!"contact_email") /\ ValidDomainName a!"sourcehost") inil))))        (SumType_index ResourceRecordTypeTypes rr!sRDATA)
         (SumType_proj ResourceRecordTypeTypes rr!sRDATA).
     intros ? H; apply H.
@@ -958,9 +958,9 @@ Section DnsPacket.
   Definition encode_rdata_Spec :=
     encode_SumType_Spec ResourceRecordTypeTypes
                         (icons (encode_CNAME_Spec)  (* CNAME; canonical name for an alias 	[RFC1035] *)
-                        (icons encode_A_Spec (* A; host address 	[RFC1035] *)
-                        (icons (encode_NS_Spec) (* NS; authoritative name server 	[RFC1035] *)
-                        (icons encode_SOA_RDATA_Spec  (* SOA rks the start of a zone of authority 	[RFC1035] *) inil)))).
+                               (icons encode_A_Spec (* A; host address 	[RFC1035] *)
+                                      (icons (encode_NS_Spec) (* NS; authoritative name server 	[RFC1035] *)
+                                             (icons encode_SOA_RDATA_Spec  (* SOA rks the start of a zone of authority 	[RFC1035] *) inil)))).
 
   Definition encode_resource_Spec(r : resourceRecord) :=
     encode_DomainName_Spec r!sNAME
@@ -1033,28 +1033,28 @@ Section DnsPacket.
     omega.
   Qed.
 
-Ltac synthesize_decoder_ext
-     transformer
-     decode_step'
-     determineHooks
-     synthesize_cache_invariant' :=
-  (* Combines tactics into one-liner. *)
-  start_synthesizing_decoder;
-  [ normalize_compose transformer;
-    repeat first [decode_step' idtac | decode_step determineHooks]
-  | cbv beta; synthesize_cache_invariant' idtac
-  |  ].
+  Ltac synthesize_decoder_ext
+       transformer
+       decode_step'
+       determineHooks
+       synthesize_cache_invariant' :=
+    (* Combines tactics into one-liner. *)
+    start_synthesizing_decoder;
+    [ normalize_compose transformer;
+      repeat first [decode_step' idtac | decode_step determineHooks]
+    | cbv beta; synthesize_cache_invariant' idtac
+    |  ].
 
-Definition ByteAlignedCorrectDecoderFor {A} {cache : Cache}
-           Invariant FormatSpec :=
-  { decodePlusCacheInv |
+  Definition ByteAlignedCorrectDecoderFor {A} {cache : Cache}
+             Invariant FormatSpec :=
+    { decodePlusCacheInv |
       exists P_inv,
-        (cache_inv_Property (snd decodePlusCacheInv) P_inv
-         -> encode_decode_correct_f (A := A) cache transformer Invariant (fun _ _ => True)
-                                    FormatSpec
-                                    (fst decodePlusCacheInv)
-                                    (snd decodePlusCacheInv))
-        /\ cache_inv_Property (snd decodePlusCacheInv) P_inv}.
+      (cache_inv_Property (snd decodePlusCacheInv) P_inv
+       -> encode_decode_correct_f (A := A) cache transformer Invariant (fun _ _ => True)
+                                  FormatSpec
+                                  (fst decodePlusCacheInv)
+                                  (snd decodePlusCacheInv))
+      /\ cache_inv_Property (snd decodePlusCacheInv) P_inv}.
 
   Arguments split1' : simpl never.
   Arguments split2' : simpl never.
@@ -1080,8 +1080,8 @@ Definition ByteAlignedCorrectDecoderFor {A} {cache : Cache}
               try rewrite !optimize_if_bind2_bool).
 
     first [ apply DecodeBindOpt2_under_bind; simpl; intros
-            | eapply optimize_under_if_bool; simpl; intros
-            | eapply optimize_under_if; simpl; intros].
+          | eapply optimize_under_if_bool; simpl; intros
+          | eapply optimize_under_if; simpl; intros].
     unfold decode_enum at 1.
     repeat (try rewrite !DecodeBindOpt2_assoc;
             try rewrite !Bool.andb_true_r;
@@ -1090,12 +1090,16 @@ Definition ByteAlignedCorrectDecoderFor {A} {cache : Cache}
             try rewrite !optimize_if_bind2_bool).
     etransitivity.
     first [ apply DecodeBindOpt2_under_bind; simpl; intros
-            | eapply optimize_under_if_bool; simpl; intros
-            | eapply optimize_under_if; simpl; intros].
+          | eapply optimize_under_if_bool; simpl; intros
+          | eapply optimize_under_if; simpl; intros].
     rewrite !DecodeBindOpt2_assoc.
     first [ apply DecodeBindOpt2_under_bind; simpl; intros
-            | eapply optimize_under_if_bool; simpl; intros
-            | eapply optimize_under_if; simpl; intros].
+          | eapply optimize_under_if_bool; simpl; intros
+          | eapply optimize_under_if; simpl; intros].
+    rewrite (If_Opt_Then_Else_DecodeBindOpt_swap (cache := dns_list_cache)).
+    first [ apply DecodeBindOpt2_under_bind; simpl; intros
+          | eapply optimize_under_if_bool; simpl; intros
+          | eapply optimize_under_if; simpl; intros].
     rewrite (If_Opt_Then_Else_DecodeBindOpt_swap (cache := dns_list_cache)).
     first [ apply DecodeBindOpt2_under_bind; simpl; intros
           | eapply optimize_under_if_bool; simpl; intros
@@ -1106,331 +1110,47 @@ Definition ByteAlignedCorrectDecoderFor {A} {cache : Cache}
           | eapply optimize_under_if; simpl; intros].
     rewrite (If_Opt_Then_Else_DecodeBindOpt_swap (cache := dns_list_cache)).
     first [ apply DecodeBindOpt2_under_bind; simpl; intros
-            | eapply optimize_under_if_bool; simpl; intros
-            | eapply optimize_under_if; simpl; intros].
+          | eapply optimize_under_if_bool; simpl; intros
+          | eapply optimize_under_if; simpl; intros].
     rewrite (If_Opt_Then_Else_DecodeBindOpt_swap (cache := dns_list_cache)).
-  first [ apply DecodeBindOpt2_under_bind; simpl; intros
-            | eapply optimize_under_if_bool; simpl; intros
-            | eapply optimize_under_if; simpl; intros].
-  rewrite (If_Opt_Then_Else_DecodeBindOpt_swap (cache := dns_list_cache)).
-  first [ apply DecodeBindOpt2_under_bind; simpl; intros
-            | eapply optimize_under_if_bool; simpl; intros
-            | eapply optimize_under_if; simpl; intros].
-  etransitivity.
-  first [ apply DecodeBindOpt2_under_bind; simpl; intros
-            | eapply optimize_under_if_bool; simpl; intros
-            | eapply optimize_under_if; simpl; intros].
-  rewrite (If_Then_Else_Bind (cache := dns_list_cache)).
-  unfold decode_enum at 1.
-  repeat (try rewrite !DecodeBindOpt2_assoc;
-          try rewrite !Bool.andb_true_r;
-          try rewrite !Bool.andb_true_l;
-          try rewrite !optimize_if_bind2;
-          try rewrite !optimize_if_bind2_bool).
-  higher_order_reflexivity.
-  set_refine_evar.
-  rewrite (If_Opt_Then_Else_DecodeBindOpt_swap (cache := dns_list_cache)).
-  unfold H; higher_order_reflexivity.
-  collapse_word addD_addD_plus.
-  collapse_word addD_addD_plus.
-  collapse_word addD_addD_plus.
-  collapse_word addD_addD_plus.
-  first [ apply DecodeBindOpt2_under_bind; simpl; intros
-        | eapply optimize_under_if_bool; simpl; intros
-        | eapply optimize_under_if; simpl; intros].
-  collapse_word addD_addD_plus.
-  collapse_word addD_addD_plus.
-  simpl.
-  higher_order_reflexivity.
+    first [ apply DecodeBindOpt2_under_bind; simpl; intros
+          | eapply optimize_under_if_bool; simpl; intros
+          | eapply optimize_under_if; simpl; intros].
+    etransitivity.
+    first [ apply DecodeBindOpt2_under_bind; simpl; intros
+          | eapply optimize_under_if_bool; simpl; intros
+          | eapply optimize_under_if; simpl; intros].
+    rewrite (If_Then_Else_Bind (cache := dns_list_cache)).
+    unfold decode_enum at 1.
+    repeat (try rewrite !DecodeBindOpt2_assoc;
+            try rewrite !Bool.andb_true_r;
+            try rewrite !Bool.andb_true_l;
+            try rewrite !optimize_if_bind2;
+            try rewrite !optimize_if_bind2_bool).
+    higher_order_reflexivity.
+    set_refine_evar.
+    rewrite (If_Opt_Then_Else_DecodeBindOpt_swap (cache := dns_list_cache)).
+    unfold H; higher_order_reflexivity.
+    collapse_word addD_addD_plus.
+    collapse_word addD_addD_plus.
+    collapse_word addD_addD_plus.
+    collapse_word addD_addD_plus.
+    first [ apply DecodeBindOpt2_under_bind; simpl; intros
+          | eapply optimize_under_if_bool; simpl; intros
+          | eapply optimize_under_if; simpl; intros].
+    collapse_word addD_addD_plus.
+    collapse_word addD_addD_plus.
+    simpl.
+    higher_order_reflexivity.
   Defined.
 
   Definition packetDecoderImpl
     := Eval simpl in (projT1 packet_decoder).
 
-  Lemma AlignedDecodeChar {C}
-        {numBytes}
-    : forall (v : Vector.t (word 8) (S numBytes))
-             (k : (word 8) -> ByteString -> CacheDecode -> option (C * ByteString * CacheDecode))
-             cd,
-    (`(a, b0, d) <- decode_word
-      (transformerUnit := ByteString_QueueTransformerOpt) (sz := 8) (build_aligned_ByteString v) cd;
-       k a b0 d) =
-    Let n := (Vector.nth v Fin.F1) in
-        k n (build_aligned_ByteString (snd (Vector_split 1 _ v))) (addD cd 8).
-Proof.
-  unfold LetIn; intros.
-  unfold decode_word, WordOpt.decode_word.
-  rewrite aligned_decode_char_eq; simpl.
-  f_equal.
-  pattern numBytes, v; apply Vector.caseS; simpl; intros.
-  reflexivity.
-Qed.
-
-Lemma AlignedDecode2Char {C}
-        {numBytes}
-    : forall (v : Vector.t (word 8) (S (S numBytes)))
-             (k : (word 16) -> ByteString -> CacheDecode -> option (C * ByteString * CacheDecode))
-             cd,
-    (`(a, b0, d) <- decode_word
-      (transformerUnit := ByteString_QueueTransformerOpt) (sz := 16) (build_aligned_ByteString v) cd;
-       k a b0 d) =
-    Let n := Core.append_word (Vector.nth v (Fin.FS Fin.F1)) (Vector.nth v Fin.F1) in
-        k n (build_aligned_ByteString (snd (Vector_split 2 _ v))) (addD cd 16).
-Proof.
-  unfold LetIn; intros.
-  unfold decode_word, WordOpt.decode_word.
-  match goal with
-    |- context[Ifopt ?Z as _ Then _ Else _] => replace Z with
-                                               (let (v', v'') := Vector_split 2 numBytes v in Some (VectorByteToWord v', build_aligned_ByteString v'')) by (symmetry; apply (@aligned_decode_char_eq' _ 1 v))
-  end.
-  unfold Vector_split, If_Opt_Then_Else, DecodeBindOpt2 at 1, If_Opt_Then_Else.
-  f_equal.
-  rewrite !Vector_nth_tl, !Vector_nth_hd.
-  erewrite VectorByteToWord_cons.
-  rewrite <- !Eqdep_dec.eq_rect_eq_dec; eauto using Peano_dec.eq_nat_dec.
-  f_equal.
-  erewrite VectorByteToWord_cons.
-  rewrite <- !Eqdep_dec.eq_rect_eq_dec; eauto using Peano_dec.eq_nat_dec.
-  Grab Existential Variables.
-  omega.
-  omega.
-Qed.
-
-Corollary AlignedDecode2Nat {C}
-        {numBytes}
-    : forall (v : Vector.t (word 8) (S (S numBytes)))
-             (k : nat -> ByteString -> CacheDecode -> option (C * ByteString * CacheDecode))
-             cd,
-    (`(a, b0, d) <- decode_nat
-      (transformerUnit := ByteString_QueueTransformerOpt) 16 (build_aligned_ByteString v) cd;
-       k a b0 d) =
-    Let n := wordToNat (Core.append_word (Vector.nth v (Fin.FS Fin.F1)) (Vector.nth v Fin.F1)) in
-        k n (build_aligned_ByteString (snd (Vector_split 2 _ v))) (addD cd 16).
-Proof.
-  unfold decode_nat; intros.
-  rewrite DecodeBindOpt2_assoc.
-  unfold DecodeBindOpt2 at 2, If_Opt_Then_Else.
-  rewrite AlignedDecode2Char.
-  reflexivity.
-Qed.
-
-Lemma optimize_under_if_opt {A ResultT}
-  : forall (a_opt : option A) (t t' : A -> ResultT) (e e' : ResultT),
-    (forall a, t a = t' a) -> e = e' ->
-    Ifopt a_opt as a Then t a Else e = Ifopt a_opt as a Then t' a Else e'.
-Proof.
-  intros; subst; eauto.
-  destruct a_opt; eauto.
-Qed.
-
-Lemma rewrite_under_LetIn
-      {A B}
-  : forall (a : A) (k k' : A -> B),
-    (forall a, k a = k' a) -> LetIn a k = LetIn a k'.
-Proof.
-  intros; unfold LetIn; eauto.
-Qed.
-
-Fixpoint Guarded_Vector_split
-         (sz n : nat)
-         {struct sz}
-  : Vector.t (word 8) n
-    -> Vector.t (word 8) (sz + (n - sz)) :=
-  match sz, n return
-        Vector.t _ n
-        -> Vector.t (word 8) (sz + (n - sz))
-  with
-  | 0, _ => fun v => (eq_rect _ (Vector.t _) v _ (minus_n_O n))
-  | S n', 0 =>
-    fun v =>
-      Vector.cons _ (wzero _) _ (Guarded_Vector_split n' _ v)
-  | S n', S sz' =>
-    fun v =>
-      Vector.cons _ (Vector.hd v) _ (Guarded_Vector_split n' _ (Vector.tl v))
-  end .
-
-Lemma le_B_Guarded_Vector_split
-      {n}
-      (b : Vector.t _ n)
-      (m : nat)
-  : {b' : ByteString | le_B b' (build_aligned_ByteString b)}.
-  eexists (build_aligned_ByteString
-             (snd (Vector_split _ _ (Guarded_Vector_split m n b)))).
-  abstract (unfold build_aligned_ByteString, le_B; simpl; omega).
-Defined.
-
-Lemma Decode_w_Measure_le_eq'':
-  forall (A B : Type) (cache : Cache) (transformer : Transformer B)
-         (A_decode : B -> CacheDecode -> option (A * B * CacheDecode))
-         (b : B) (cd : CacheDecode)
-         (A_decode_le : forall (b0 : B) (cd0 : CacheDecode) (a : A) (b' : B) (cd' : CacheDecode),
-             A_decode b0 cd0 = Some (a, b', cd') -> le_B b' b0),
-    Decode_w_Measure_le A_decode b cd A_decode_le = None ->
-    A_decode b cd = None.
-Proof.
-  clear; intros ? ? ? ? ? ? ? ?; unfold Decode_w_Measure_le in *.
-  remember (A_decode_le b cd); clear Heql.
-  destruct (A_decode b cd) as [ [ [? ?] ? ] | ]; eauto.
-  intros; discriminate.
-Qed.
-
-Lemma build_aligned_ByteString_eq_split
-  : forall m n b H0,
-    (m <= n)%nat
-    -> build_aligned_ByteString b =
-       (build_aligned_ByteString (eq_rect (m + (n - m)) (t (word 8)) (Guarded_Vector_split m n b) n H0)).
-Proof.
-  intros.
-  intros; eapply ByteString_f_equal; simpl.
-  instantiate (1 := eq_refl _); reflexivity.
-  instantiate (1 := eq_refl _).
-  simpl.
-  revert n b H0 H; induction m; simpl.
-  intros ? ?; generalize (minus_n_O n).
-  intros; rewrite <- Equality.transport_pp.
-  apply Eqdep_dec.eq_rect_eq_dec; auto with arith.
-  intros.
-  inversion H; subst.
-  - revert b H0 IHm; clear.
-    intro; pattern m, b; apply Vector.caseS; simpl; intros.
-    assert ((n + (n - n)) = n) by omega.
-    rewrite eq_rect_Vector_cons with (H' := H).
-    f_equal.
-    erewrite <- IHm; eauto.
-  - revert b H0 IHm H1; clear.
-    intro; pattern m0, b; apply Vector.caseS; simpl; intros.
-    assert ((m + (n - m)) = n) by omega.
-    erewrite eq_rect_Vector_cons with (H' := H).
-    f_equal.
-    erewrite <- IHm; eauto.
-    omega.
-Qed.
-
-Lemma ByteAlign_Decode_w_Measure_le {A}
-  : forall (dec_a : ByteString -> CacheDecode -> option (A * ByteString * CacheDecode))
-           (n m : nat)
-           (dec_a' : Vector.t (word 8) (m + (n - m)) -> A)
-           (cd : CacheDecode)
-           (f : CacheDecode -> CacheDecode)
-           (b : Vector.t (word 8) n)
-           decode_a_le
-           (dec_fail : ~ (m <= n)%nat
-                       -> forall b cd, dec_a (build_aligned_ByteString (numBytes := n) b) cd = None),
-    (forall b cd, dec_a (build_aligned_ByteString b) cd =
-                  Some (dec_a' b, build_aligned_ByteString (snd (Vector_split m (n - m) b)), f cd))
-    -> Decode_w_Measure_le dec_a (build_aligned_ByteString b) cd decode_a_le =
-       match Compare_dec.le_dec m n with
-       | left e => (Let a := dec_a' (Guarded_Vector_split m n b) in
-                        Some (a, le_B_Guarded_Vector_split b m, f cd))
-       | right _ => None
-       end.
-Proof.
-  intros.
-  destruct (Compare_dec.le_dec m n).
-  assert (m + (n - m) = n) by omega.
-  assert (forall b, Decode_w_Measure_le dec_a (build_aligned_ByteString b) cd decode_a_le
-                    = Decode_w_Measure_le dec_a (build_aligned_ByteString ( eq_rect _ _ (Guarded_Vector_split m n b) _ H0)) cd decode_a_le).
-  { revert l; clear; intros.
-    destruct (Decode_w_Measure_le dec_a (build_aligned_ByteString b) cd decode_a_le)
-      as [ [ [? [? ?] ] ?] | ] eqn: ?.
-    apply Decode_w_Measure_le_eq' in Heqo.
-    simpl in Heqo.
-    destruct (Decode_w_Measure_le dec_a
-                                  (build_aligned_ByteString (eq_rect (m + (n - m)) (t (word 8)) (Guarded_Vector_split m n b) n H0)) cd decode_a_le) as [ [ [? [? ?] ] ?] | ] eqn: ?.
-    apply Decode_w_Measure_le_eq' in Heqo0.
-    simpl in *.
-    rewrite <- build_aligned_ByteString_eq_split in Heqo0 by eauto.
-    rewrite Heqo0 in Heqo.
-    injection Heqo; intros.
-    rewrite H, H2;
-      repeat f_equal.
-    revert l0 l1. rewrite H1; intros; f_equal.
-    f_equal; apply Core.le_uniqueness_proof.
-    apply ByteString_id.
-    eapply Decode_w_Measure_le_eq'' in Heqo0.
-    rewrite <- build_aligned_ByteString_eq_split in Heqo0 by eauto.
-    rewrite Heqo0 in Heqo.
-    discriminate.
-    apply ByteString_id.
-    erewrite build_aligned_ByteString_eq_split in Heqo by eauto.
-    rewrite Heqo; reflexivity.
-  }
-  rewrite H1.
-  match goal with
-    |- ?a = _ => destruct a as [ [ [? ?] ? ] | ] eqn: ?
-  end.
-  eapply Decode_w_Measure_le_eq' in Heqo.
-  assert (dec_a (build_aligned_ByteString (Guarded_Vector_split m n b)) cd
-          = Some (a, projT1 s, c)).
-  { destruct s; simpl in *.
-    rewrite <- Heqo.
-    unfold build_aligned_ByteString; repeat f_equal; simpl.
-    eapply ByteString_f_equal; simpl.
-    instantiate (1 := eq_refl _); reflexivity.
-    instantiate (1 := sym_eq H0).
-    clear H1.
-    destruct H0; reflexivity.
-  }
-  rewrite H in H2; injection H2; intros.
-  rewrite H3, H5; unfold LetIn; simpl.
-  repeat f_equal.
-  destruct s; simpl in *.
-  unfold le_B_Guarded_Vector_split; simpl.
-  clear H1; revert l0.
-  rewrite <- H4; intros.
-  f_equal; apply Core.le_uniqueness_proof.
-  apply ByteString_id.
-  apply Decode_w_Measure_le_eq'' in Heqo.
-  pose proof (H (Guarded_Vector_split m n b) cd).
-  assert (Some (dec_a' (Guarded_Vector_split m n b),
-                build_aligned_ByteString (snd (Vector_split m (n - m) (Guarded_Vector_split m n b))),
-                f cd) = None).
-  { rewrite <- Heqo.
-    rewrite <- H.
-    repeat f_equal.
-    eapply ByteString_f_equal; simpl.
-    instantiate (1 := eq_refl _); reflexivity.
-    instantiate (1 := sym_eq H0).
-    clear H1.
-    destruct H0; reflexivity.
-  }
-  discriminate.
-  eapply dec_fail in n0; simpl.
-  eapply Specs.Decode_w_Measure_le_eq' in n0.
-  apply n0.
-Qed.
-
-Lemma lt_B_Guarded_Vector_split
-      {n}
-      (b : Vector.t _ n)
-      (m : nat)
-      (m_OK : lt 0 m)
-      (_ : ~ lt n m)
-  : {b' : ByteString | lt_B b' (build_aligned_ByteString b)}.
-  eexists (build_aligned_ByteString
-             (snd (Vector_split _ _ (Guarded_Vector_split m n b)))).
-  abstract (unfold build_aligned_ByteString, lt_B; simpl; omega).
-Defined.
-
-Lemma Decode_w_Measure_lt_eq'':
-  forall (A B : Type) (cache : Cache) (transformer : Transformer B)
-         (A_decode : B -> CacheDecode -> option (A * B * CacheDecode))
-         (b : B) (cd : CacheDecode)
-         (A_decode_lt : forall (b0 : B) (cd0 : CacheDecode) (a : A) (b' : B) (cd' : CacheDecode),
-             A_decode b0 cd0 = Some (a, b', cd') -> lt_B b' b0),
-    Decode_w_Measure_lt A_decode b cd A_decode_lt = None ->
-    A_decode b cd = None.
-Proof.
-  clear; intros ? ? ? ? ? ? ? ?; unfold Decode_w_Measure_lt in *.
-  remember (A_decode_lt b cd); clear Heql.
-  destruct (A_decode b cd) as [ [ [? ?] ? ] | ]; eauto.
-  discriminate.
-Qed.
-
-Arguments Guarded_Vector_split : simpl never.
+  Arguments Guarded_Vector_split : simpl never.
 
   Fixpoint BytesToString {sz}
-             (b : Vector.t (word 8) sz)
+           (b : Vector.t (word 8) sz)
     : string :=
     match b with
     | Vector.nil => EmptyString
@@ -1439,356 +1159,6 @@ Arguments Guarded_Vector_split : simpl never.
 
   Arguments addD : simpl never.
 
-  Lemma decode_string_aligned_ByteString
-        {sz sz'}
-    : forall (b : t (word 8) (sz + sz'))
-        (cd : CacheDecode),
-  FixStringOpt.decode_string sz (build_aligned_ByteString b) cd =
-  Some (BytesToString (fst (Vector_split sz sz' b)),
-        build_aligned_ByteString (snd (Vector_split sz sz' b)),
-        addD cd (8 * sz)).
-  Proof.
-    induction sz; intros.
-    - simpl; repeat f_equal.
-      destruct cd as [ [? | ] ? ]; unfold addD; simpl.
-      pose proof (wordToNat_bound w); find_if_inside; try omega.
-      rewrite plus_comm; simpl; rewrite natToWord_wordToNat; reflexivity.
-      reflexivity.
-    - simpl.
-      assert (forall A n b, exists a b', b = Vector.cons A a n b')
-             by (clear; intros; pattern n, b; apply caseS; eauto).
-      destruct (H _ _ b) as [? [? ?] ]; subst; simpl.
-      unfold AsciiOpt.decode_ascii.
-      rewrite DecodeBindOpt2_assoc; simpl.
-      etransitivity.
-      rewrite AlignedDecodeChar; simpl.
-      rewrite IHsz. higher_order_reflexivity.
-      simpl.
-      destruct (Vector_split sz sz' x0); simpl.
-      unfold LetIn.
-      rewrite addD_addD_plus;
-        repeat f_equal.
-      omega.
-  Qed.
-
-  Lemma decode_string_aligned_ByteString_overflow
-        {sz}
-    : forall {sz'}
-             (b : t (word 8) sz')
-             (cd : CacheDecode),
-             lt sz' sz
-             -> FixStringOpt.decode_string sz (build_aligned_ByteString b) cd = None.
-  Proof.
-    induction sz; intros.
-    - omega.
-    - simpl.
-      assert (forall A n b, exists a b', b = Vector.cons A a n b')
-             by (clear; intros; pattern n, b; apply caseS; eauto).
-      destruct sz'.
-      + reflexivity.
-      + destruct (H0 _ _ b) as [? [? ?] ]; subst; simpl.
-        unfold AsciiOpt.decode_ascii.
-        rewrite DecodeBindOpt2_assoc; simpl.
-        etransitivity.
-        rewrite AlignedDecodeChar; simpl.
-        rewrite IHsz. higher_order_reflexivity.
-        omega.
-        reflexivity.
-  Qed.
-
-Lemma ByteAlign_Decode_w_Measure_lt {A}
-  : forall (dec_a : nat -> ByteString -> CacheDecode -> option (A * ByteString * CacheDecode))
-           (n m : nat)
-           (dec_a' : forall m n, Vector.t (word 8) (m + n) -> A)
-           (cd : CacheDecode)
-           (f : nat -> CacheDecode -> CacheDecode)
-           (b : Vector.t (word 8) n)
-           (m_OK : lt 0 m)
-           decode_a_le
-           (dec_fail : (lt n m)%nat
-                       -> forall b cd, dec_a m (build_aligned_ByteString (numBytes := n) b) cd = None),
-    (forall n m b cd, dec_a m (build_aligned_ByteString b) cd =
-                      Some (dec_a' _ _ b, build_aligned_ByteString (snd (Vector_split m n b)), f m cd))
-    -> Decode_w_Measure_lt (dec_a m) (build_aligned_ByteString b) cd decode_a_le =
-       match Compare_dec.lt_dec n m with
-       | left _ => None
-       | right n' => (Let a := dec_a' _ _ (Guarded_Vector_split m n b) in
-                         Some (a, lt_B_Guarded_Vector_split b m m_OK n' , f m cd))
-       end.
-Proof.
-  intros.
-  destruct (Compare_dec.lt_dec m n);
-    destruct (Compare_dec.lt_dec n m); try omega.
-  - assert (m + (n - m) = n) by omega.
-    assert (forall b, Decode_w_Measure_lt (dec_a m) (build_aligned_ByteString b) cd decode_a_le
-                      = Decode_w_Measure_lt (dec_a m)(build_aligned_ByteString ( eq_rect _ _ (Guarded_Vector_split m n b) _ H0)) cd decode_a_le).
-    { revert l; clear; intros.
-      destruct (Decode_w_Measure_lt (dec_a m) (build_aligned_ByteString b) cd decode_a_le)
-        as [ [ [? [? ?] ] ?] | ] eqn: ?.
-      apply Decode_w_Measure_lt_eq' in Heqo.
-      simpl in Heqo.
-      destruct (Decode_w_Measure_lt (dec_a m)
-                                    (build_aligned_ByteString (eq_rect _ (t (word 8)) (Guarded_Vector_split m n b) n H0)) cd decode_a_le) as [ [ [? [? ?] ] ?] | ] eqn: ?.
-      apply Decode_w_Measure_lt_eq' in Heqo0.
-      unfold proj1_sig in Heqo0.
-      rewrite <- build_aligned_ByteString_eq_split in Heqo0.
-      rewrite Heqo0 in Heqo.
-      injection Heqo; intros.
-      rewrite H, H2;
-        repeat f_equal.
-      revert l1 l0. rewrite H1; intros; f_equal.
-      f_equal; apply Core.le_uniqueness_proof.
-      omega.
-      apply ByteString_id.
-      eapply Decode_w_Measure_lt_eq'' in Heqo0.
-      rewrite <- build_aligned_ByteString_eq_split in Heqo0 by omega.
-      rewrite Heqo0 in Heqo.
-      discriminate.
-      apply ByteString_id.
-      erewrite (build_aligned_ByteString_eq_split m n) in Heqo by omega.
-      rewrite Heqo; reflexivity.
-    }
-    rewrite H1.
-    match goal with
-      |- ?a = _ => destruct a as [ [ [? ?] ? ] | ] eqn: ?
-    end.
-    eapply Decode_w_Measure_lt_eq' in Heqo.
-    assert (dec_a m (build_aligned_ByteString (Guarded_Vector_split m n b)) cd
-            = Some (a, projT1 s, c)).
-    { destruct s; simpl in *.
-      rewrite <- Heqo.
-      unfold build_aligned_ByteString; repeat f_equal; simpl.
-      eapply ByteString_f_equal; simpl.
-      instantiate (1 := eq_refl _); reflexivity.
-      instantiate (1 := sym_eq H0).
-      clear H1.
-      destruct H0; reflexivity.
-    }
-    rewrite H in H2; injection H2; intros.
-    rewrite H3, H5; unfold LetIn; simpl.
-    repeat f_equal.
-    destruct s; simpl in *.
-    unfold lt_B_Guarded_Vector_split; simpl.
-    clear H1; revert l0.
-    rewrite <- H4; intros.
-    f_equal. apply Core.le_uniqueness_proof.
-    apply ByteString_id.
-    apply Decode_w_Measure_lt_eq'' in Heqo.
-    pose proof (H _ _ (Guarded_Vector_split m n b) cd).
-    assert (Some (dec_a' _ _ (Guarded_Vector_split m n b),
-                  build_aligned_ByteString (snd (Vector_split m (n - m) (Guarded_Vector_split m n b))),
-                  f m cd) = None).
-    { rewrite <- Heqo.
-      rewrite <- H.
-      repeat f_equal.
-      eapply ByteString_f_equal; simpl.
-      instantiate (1 := eq_refl _); reflexivity.
-      instantiate (1 := sym_eq H0).
-      clear H1.
-      destruct H0; reflexivity.
-    }
-    discriminate.
-  - eapply dec_fail in l; simpl.
-    eapply Specs.Decode_w_Measure_lt_eq' in l.
-    apply l.
-  - assert (m = n) by omega; subst.
-    assert (n + (n - n) = n) by omega.
-    assert (forall b, Decode_w_Measure_lt (dec_a n) (build_aligned_ByteString b) cd decode_a_le
-                      = Decode_w_Measure_lt (dec_a n)(build_aligned_ByteString ( eq_rect _ _ (Guarded_Vector_split n n b) _ H0)) cd decode_a_le).
-    { clear; intros.
-      destruct (Decode_w_Measure_lt (dec_a n) (build_aligned_ByteString b) cd decode_a_le)
-        as [ [ [? [? ?] ] ?] | ] eqn: ?.
-      apply Decode_w_Measure_lt_eq' in Heqo.
-      simpl in Heqo.
-      destruct (Decode_w_Measure_lt (dec_a n)
-                                    (build_aligned_ByteString (eq_rect _ (t (word 8)) (Guarded_Vector_split n n b) n H0)) cd decode_a_le) as [ [ [? [? ?] ] ?] | ] eqn: ?.
-    apply Decode_w_Measure_lt_eq' in Heqo0.
-    unfold proj1_sig in Heqo0.
-    rewrite <- build_aligned_ByteString_eq_split in Heqo0.
-    rewrite Heqo0 in Heqo.
-    injection Heqo; intros.
-    rewrite H, H2;
-      repeat f_equal.
-    revert l l0. rewrite H1; intros; f_equal.
-    f_equal; apply Core.le_uniqueness_proof.
-    omega.
-    apply ByteString_id.
-    eapply Decode_w_Measure_lt_eq'' in Heqo0.
-    rewrite <- build_aligned_ByteString_eq_split in Heqo0 by omega.
-    rewrite Heqo0 in Heqo.
-    discriminate.
-    apply ByteString_id.
-    erewrite (build_aligned_ByteString_eq_split n n) in Heqo by omega.
-    rewrite Heqo; reflexivity.
-  }
-  rewrite H1.
-  match goal with
-    |- ?a = _ => destruct a as [ [ [? ?] ? ] | ] eqn: ?
-  end.
-  eapply Decode_w_Measure_lt_eq' in Heqo.
-  assert (dec_a n (build_aligned_ByteString (Guarded_Vector_split n n b)) cd
-          = Some (a, projT1 s, c)).
-  { destruct s; simpl in *.
-    rewrite <- Heqo.
-    unfold build_aligned_ByteString; repeat f_equal; simpl.
-    eapply ByteString_f_equal; simpl.
-    instantiate (1 := eq_refl _); reflexivity.
-    instantiate (1 := sym_eq H0).
-    clear H1.
-    destruct H0; reflexivity.
-  }
-  rewrite H in H2; injection H2; intros.
-  rewrite H3, H5; unfold LetIn; simpl.
-  repeat f_equal.
-  destruct s; simpl in *.
-  unfold lt_B_Guarded_Vector_split; simpl.
-  clear H1; revert l.
-  rewrite <- H4; intros.
-  f_equal. apply Core.le_uniqueness_proof.
-  apply ByteString_id.
-  apply Decode_w_Measure_lt_eq'' in Heqo.
-  pose proof (H _ _ (Guarded_Vector_split n n b) cd).
-  assert (Some (dec_a' _ _ (Guarded_Vector_split n n b),
-                build_aligned_ByteString (snd (Vector_split n (n - n) (Guarded_Vector_split n n b))),
-                f n cd) = None).
-  { rewrite <- Heqo.
-    rewrite <- H.
-    repeat f_equal.
-    eapply ByteString_f_equal; simpl.
-    instantiate (1 := eq_refl _); reflexivity.
-    instantiate (1 := sym_eq H0).
-    clear H1.
-    destruct H0; reflexivity.
-  }
-  discriminate.
-Qed.
-
-  Lemma optimize_If_bind2_bool {A A' B B' C}
-    : forall (c : bool)
-             (t e : option (A * B * C))
-             (k : A -> B -> C -> option (A' * B' * C)),
-      (`(a, b, env) <- (If c Then t Else e); k a b env) =
-      If c Then `(a, b, env) <- t; k a b env Else (`(a, b, env) <- e; k a b env).
-  Proof.
-    destruct c; simpl; intros; reflexivity.
-  Qed.
-
-  Lemma optimize_under_match {A B} {P}
-    : forall (a a' : A) (f : {P a a'} + {~P a a'}) (t t' : _ -> B)
-             (e e' : _ -> B),
-      (forall (a a' : A) (a_eq : _), t a_eq = t' a_eq)
-      -> (forall (a a' : A) (a_neq : _), e a_neq = e' a_neq)
-      -> match f with
-          | left e => t e
-          | right n => e n
-         end =
-         match f with
-         | left e => t' e
-         | right n => e' n
-         end.
-  Proof.
-    destruct f; simpl; intros; eauto.
-  Qed.
-
-Lemma optimize_Fix {A}
-  : forall
-    (body : forall x : ByteString,
-        (forall y : ByteString,
-            lt_B y x -> (fun _ : ByteString => CacheDecode -> option (A * ByteString * CacheDecode)) y) ->
-        (fun _ : ByteString => CacheDecode -> option (A * ByteString * CacheDecode)) x)
-    (body' : forall x : nat,
-        (forall y : nat,
-            (lt y x)%nat ->
-            (fun m : nat =>
-               t (word 8) m -> CacheDecode ->
-               option (A * {n : _ & Vector.t _ n} * CacheDecode)) y) ->
-        t (word 8) x -> CacheDecode -> option (A * {n : _ & Vector.t _ n} * CacheDecode) )
-    n (b : Vector.t _ n) (cd : CacheDecode)
-    (body_Proper :
-       forall (x0 : ByteString)
-              (f g : forall y : ByteString, lt_B y x0 -> CacheDecode -> option (A * ByteString * CacheDecode)),
-         (forall (y : ByteString) (p : lt_B y x0), f y p = g y p) -> body x0 f = body x0 g)
-    (body'_Proper :
-       forall (x0 : nat)
-              (f
-                 g : forall y : nat,
-                  (lt y x0)%nat -> t (word 8) y -> CacheDecode -> option (A * {n0 : nat & t Core.char n0} * CacheDecode)),
-         (forall (y : nat) (p : (lt y x0)%nat), f y p = g y p) -> body' x0 f = body' x0 g)
-  ,
-    (forall n (b : Vector.t (word 8) n)
-            (rec : forall x : ByteString,
-                lt_B x (build_aligned_ByteString b) -> CacheDecode -> option (A * ByteString * CacheDecode))
-            (rec' : forall x : nat,
-                (lt x n)%nat -> t Core.char x -> CacheDecode ->
-                option (A * {n : _ & Vector.t _ n} * CacheDecode))
-            cd,
-        (forall m cd b a b' cd' b_lt b_lt' ,
-            rec' m b_lt' b cd = Some (a, b', cd')
-            -> rec (build_aligned_ByteString b) b_lt cd = Some (a, build_aligned_ByteString (projT2 b'), cd'))
-        -> (forall m cd b b_lt b_lt' ,
-            rec' m b_lt' b cd = None
-            -> rec (build_aligned_ByteString b) b_lt cd = None)
-        -> body (build_aligned_ByteString b) rec cd
-           = match (body' n rec' b cd) with
-             | Some (a, b', cd') => Some (a, build_aligned_ByteString (projT2 b'), cd')
-             | None => None
-             end)
-    -> Fix well_founded_lt_b (fun _ : ByteString => CacheDecode -> option (A * ByteString * CacheDecode)) body (build_aligned_ByteString b) cd =
-       match Fix Wf_nat.lt_wf (fun m : nat => Vector.t (word 8) m -> CacheDecode -> option (A * { n : _ & Vector.t _ n} * CacheDecode)) body' n b cd with
-       | Some (a, b', cd') => Some (a, build_aligned_ByteString (projT2 b'), cd')
-       | None => None
-       end.
-Proof.
-  intros.
-  revert cd b; pattern n.
-  eapply (well_founded_ind Wf_nat.lt_wf); intros.
-  rewrite Init.Wf.Fix_eq, Init.Wf.Fix_eq.
-  apply H; intros.
-  erewrite H0, H1; eauto.
-  rewrite H0, H1; eauto.
-  eauto.
-  eauto.
-Qed.
-
-Lemma If_sumbool_Then_Else_DecodeBindOpt {A B B' ResultT ResultT'} {P}
-  : forall (a_eq_dec : forall a a' : A, {P a a'} + {~ P a a'})
-           a a'
-           (k : _ -> _ -> _ -> option (ResultT' * B' * CacheDecode))
-           (t : P a a' ->  option (ResultT * B * CacheDecode))
-           (e : ~ P a a' -> option (ResultT * B * CacheDecode)),
-    (`(w, b', cd') <- match a_eq_dec a a' with
-                      | left e => t e
-                      | right n => e n
-                      end;
-       k w b' cd') =
-    match a_eq_dec a a' with
-    | left e => `(w, b', cd') <- t e; k w b' cd'
-    | right n => `(w, b', cd') <- e n; k w b' cd'
-    end.
-Proof.
-  intros; destruct (a_eq_dec a a'); simpl; intros; reflexivity.
-Qed.
-
-Lemma optimize_under_DecodeBindOpt2_both {A B C D E} {B' }
-  : forall (a_opt : option (A * B * C))
-           (a_opt' : option (A * B' * C))
-           (g : B' -> B)
-           (a_opt_eq_Some : forall a' b' c,
-               a_opt' = Some (a', b', c) ->
-               a_opt = Some (a', g b', c))
-           (a_opt_eq_None : a_opt' = None -> a_opt = None)
-           (k : _ -> _ -> _ -> option (D * E * C))
-           (k' : _ -> _ -> _ -> _)
-           (k_eq_Some :
-              forall a' b' c,
-                a_opt' = Some (a', b', c) ->
-                k a' (g b') c = k' a' b' c),
-    DecodeBindOpt2 a_opt k = DecodeBindOpt2 a_opt' k'.
-Proof.
-  destruct a_opt' as [ [ [? ?] ?] | ]; simpl; intros.
-  erewrite a_opt_eq_Some; simpl; eauto.
-  erewrite a_opt_eq_None; simpl; eauto.
-  Qed.
 
   Lemma rec_aligned_decode_DomainName_OK
     : forall (x : nat) (x0 : t (word 8) x),
@@ -1804,709 +1174,294 @@ Proof.
              (cd : CacheDecode) :=
     let body :=
         fun n0
-                  (rec' : forall x : nat,
-                      (lt x n0)%nat ->
-                      t Core.char x -> CacheDecode -> option (RRecordTypes.DomainName * {n1 : nat & t Core.char n1} * CacheDecode))
-                  b cd =>
+            (rec' : forall x : nat,
+                (lt x n0)%nat ->
+                t Core.char x -> CacheDecode -> option (RRecordTypes.DomainName * {n1 : nat & t Core.char n1} * CacheDecode))
+            b cd =>
           match Compare_dec.le_dec 1 n0 with
-       | left e1 =>
-     match wlt_dec (natToWord 8 191) (Vector.hd (Guarded_Vector_split 1 n0 b)) with
-     | left e =>
-         if match n0 - 1 with
-            | 0 => false
-            | S _ => true
+          | left e1 =>
+            match wlt_dec (natToWord 8 191) (Vector.hd (Guarded_Vector_split 1 n0 b)) with
+            | left e =>
+              if match n0 - 1 with
+                 | 0 => false
+                 | S _ => true
+                 end
+              then
+                match
+                  association_list_find_first (snd cd)
+                                              (exist (wlt (natToWord 8 191)) (Vector.hd (Guarded_Vector_split 1 n0 b)) e,
+                                               Vector.hd (Guarded_Vector_split 1 (n0 - 1) (Vector.tl (Guarded_Vector_split 1 n0 b))))
+                with
+                | Some ""%string => None
+                | Some (String _ _ as domain) =>
+                  Some
+                    (domain,
+                     existT (fun n => Vector.t (word 8) n) _ (Vector.tl (Guarded_Vector_split 1 (n0 - 1) (Vector.tl (Guarded_Vector_split 1 n0 b)))),
+                     addD (addD cd 8) 8)
+                | None => None
+                end
+              else None
+            | right n1 =>
+              if bool_of_sumbool (wlt_dec (Vector.hd (Guarded_Vector_split 1 n0 b)) (natToWord 8 64))
+              then
+                match weq (Vector.hd (Guarded_Vector_split 1 n0 b)) (wzero 8) with
+                | in_left => Some (""%string, existT (fun n => Vector.t (word 8) n) _ (Vector.tl (Guarded_Vector_split 1 n0 b)), addD cd 8)
+                | right n2 =>
+                  (fun a_neq0 : Vector.hd (Guarded_Vector_split 1 n0 b) <> wzero 8 =>
+                     match Compare_dec.lt_dec (n0 - 1) (wordToNat (Vector.hd (Guarded_Vector_split 1 n0 b))) with
+                     | left e => (fun _ : lt (n0 - 1) (wordToNat (Vector.hd (Guarded_Vector_split 1 n0 b)))%nat => None) e
+                     | right n3 =>
+                       (fun a_neq1 : ~ lt (n0 - 1) (wordToNat (Vector.hd (Guarded_Vector_split 1 n0 b)))%nat =>
+                          Ifopt index 0 "."
+                                (BytesToString
+                                   (fst
+                                      (Vector_split (wordToNat (Vector.hd (Guarded_Vector_split 1 n0 b)))
+                                                    (n0 - 1 - wordToNat (Vector.hd (Guarded_Vector_split 1 n0 b)))
+                                                    (Guarded_Vector_split
+                                                       (wordToNat (Vector.hd (Guarded_Vector_split 1 n0 b)))
+                                                       (n0 - 1) (Vector.tl (Guarded_Vector_split 1 n0 b)))))) as a8 Then
+                                                                                                                    (fun _ : nat => None) a8
+                                                                                                                    Else (`(d, s, c) <- rec' (n0 - 1 - wordToNat (Vector.hd (Guarded_Vector_split 1 n0 b)))
+                                                                                                                           (rec_aligned_decode_DomainName_OK n0 b e1 n3)
+                                                                                                                           (snd
+                                                                                                                              (Vector_split
+                                                                                                                                 (wordToNat (Vector.hd (Guarded_Vector_split 1 n0 b)))
+                                                                                                                                 (n0 - 1 - wordToNat (Vector.hd (Guarded_Vector_split 1 n0 b)))
+                                                                                                                                 (Guarded_Vector_split
+                                                                                                                                    (wordToNat (Vector.hd (Guarded_Vector_split 1 n0 b)))
+                                                                                                                                    (n0 - 1)
+                                                                                                                                    (Vector.tl (Guarded_Vector_split 1 n0 b)))))
+                                                                                                                           (addD (addD cd 8) (8 * wordToNat (Vector.hd (Guarded_Vector_split 1 n0 b))));
+                                                                                                                            If string_dec d ""
+                                                                                                                               Then Some
+                                                                                                                               (BytesToString
+                                                                                                                                  (fst
+                                                                                                                                     (Vector_split
+                                                                                                                                        (wordToNat (Vector.hd (Guarded_Vector_split 1 n0 b)))
+                                                                                                                                        (n0 - 1 - wordToNat (Vector.hd (Guarded_Vector_split 1 n0 b)))
+                                                                                                                                        (Guarded_Vector_split
+                                                                                                                                           (wordToNat (Vector.hd (Guarded_Vector_split 1 n0 b)))
+                                                                                                                                           (n0 - 1)
+                                                                                                                                           (Vector.tl (Guarded_Vector_split 1 n0 b))))),
+                                                                                                                                s,
+                                                                                                                                Ifopt Ifopt fst cd as m Then Some (Nat2pointerT (wordToNat (wtl (wtl (wtl m))))) Else None
+                                                                                                                                   as curPtr
+                                                                                                                                        Then (fst c,
+                                                                                                                                              ((curPtr,
+                                                                                                                                                BytesToString
+                                                                                                                                                  (fst
+                                                                                                                                                     (Vector_split
+                                                                                                                                                        (wordToNat (Vector.hd (Guarded_Vector_split 1 n0 b)))
+                                                                                                                                                        (n0 - 1 - wordToNat (Vector.hd (Guarded_Vector_split 1 n0 b)))
+                                                                                                                                                        (Guarded_Vector_split
+                                                                                                                                                           (wordToNat (Vector.hd (Guarded_Vector_split 1 n0 b)))
+                                                                                                                                                           (n0 - 1)
+                                                                                                                                                           (Vector.tl (Guarded_Vector_split 1 n0 b)))))) ::
+                                                                                                                                                                                                         snd c)%list) Else c)
+                                                                                                                               Else Some
+                                                                                                                               ((BytesToString
+                                                                                                                                   (fst
+                                                                                                                                      (Vector_split
+                                                                                                                                         (wordToNat (Vector.hd (Guarded_Vector_split 1 n0 b)))
+                                                                                                                                         (n0 - 1 - wordToNat (Vector.hd (Guarded_Vector_split 1 n0 b)))
+                                                                                                                                         (Guarded_Vector_split
+                                                                                                                                            (wordToNat (Vector.hd (Guarded_Vector_split 1 n0 b)))
+                                                                                                                                            (n0 - 1)
+                                                                                                                                            (Vector.tl (Guarded_Vector_split 1 n0 b))))) ++
+                                                                                                                                   String "." d)%string,
+                                                                                                                                s,
+                                                                                                                                Ifopt Ifopt fst cd as m Then Some (Nat2pointerT (wordToNat (wtl (wtl (wtl m))))) Else None
+                                                                                                                                   as curPtr
+                                                                                                                                        Then (fst c,
+                                                                                                                                              ((curPtr,
+                                                                                                                                                (BytesToString
+                                                                                                                                                   (fst
+                                                                                                                                                      (Vector_split
+                                                                                                                                                         (wordToNat (Vector.hd (Guarded_Vector_split 1 n0 b)))
+                                                                                                                                                         (n0 - 1 - wordToNat (Vector.hd (Guarded_Vector_split 1 n0 b)))
+                                                                                                                                                         (Guarded_Vector_split
+                                                                                                                                                            (wordToNat (Vector.hd (Guarded_Vector_split 1 n0 b)))
+                                                                                                                                                            (n0 - 1)
+                                                                                                                                                            (Vector.tl (Guarded_Vector_split 1 n0 b))))) ++
+                                                                                                                                                   String "." d)%string) ::
+                                                                                                                                                                         snd c)%list) Else c))) n3
+                     end) n2
+                end
+              else None
             end
-         then
-          match
-            association_list_find_first (snd cd)
-              (exist (wlt (natToWord 8 191)) (Vector.hd (Guarded_Vector_split 1 n0 b)) e,
-              Vector.hd (Guarded_Vector_split 1 (n0 - 1) (Vector.tl (Guarded_Vector_split 1 n0 b))))
-          with
-          | Some ""%string => None
-          | Some (String _ _ as domain) =>
-              Some
-                (domain,
-                 existT (fun n => Vector.t (word 8) n) _ (Vector.tl (Guarded_Vector_split 1 (n0 - 1) (Vector.tl (Guarded_Vector_split 1 n0 b)))),
-                addD (addD cd 8) 8)
-          | None => None
-          end
-         else None
-     | right n1 =>
-         if bool_of_sumbool (wlt_dec (Vector.hd (Guarded_Vector_split 1 n0 b)) (natToWord 8 64))
-         then
-          match weq (Vector.hd (Guarded_Vector_split 1 n0 b)) (wzero 8) with
-          | in_left => Some (""%string, existT (fun n => Vector.t (word 8) n) _ (Vector.tl (Guarded_Vector_split 1 n0 b)), addD cd 8)
-          | right n2 =>
-              (fun a_neq0 : Vector.hd (Guarded_Vector_split 1 n0 b) <> wzero 8 =>
-               match Compare_dec.lt_dec (n0 - 1) (wordToNat (Vector.hd (Guarded_Vector_split 1 n0 b))) with
-               | left e => (fun _ : lt (n0 - 1) (wordToNat (Vector.hd (Guarded_Vector_split 1 n0 b)))%nat => None) e
-               | right n3 =>
-                   (fun a_neq1 : ~ lt (n0 - 1) (wordToNat (Vector.hd (Guarded_Vector_split 1 n0 b)))%nat =>
-                    Ifopt index 0 "."
-                            (BytesToString
-                               (fst
-                                  (Vector_split (wordToNat (Vector.hd (Guarded_Vector_split 1 n0 b)))
-                                     (n0 - 1 - wordToNat (Vector.hd (Guarded_Vector_split 1 n0 b)))
-                                     (Guarded_Vector_split
-                                        (wordToNat (Vector.hd (Guarded_Vector_split 1 n0 b)))
-                                        (n0 - 1) (Vector.tl (Guarded_Vector_split 1 n0 b)))))) as a8 Then
-                    (fun _ : nat => None) a8
-                    Else (`(d, s, c) <- rec' (n0 - 1 - wordToNat (Vector.hd (Guarded_Vector_split 1 n0 b)))
-                                          (rec_aligned_decode_DomainName_OK n0 b e1 n3)
-                                          (snd
-                                             (Vector_split
-                                                (wordToNat (Vector.hd (Guarded_Vector_split 1 n0 b)))
-                                                (n0 - 1 - wordToNat (Vector.hd (Guarded_Vector_split 1 n0 b)))
-                                                (Guarded_Vector_split
-                                                  (wordToNat (Vector.hd (Guarded_Vector_split 1 n0 b)))
-                                                  (n0 - 1)
-                                                  (Vector.tl (Guarded_Vector_split 1 n0 b)))))
-                                          (addD (addD cd 8) (8 * wordToNat (Vector.hd (Guarded_Vector_split 1 n0 b))));
-                          If string_dec d ""
-                          Then Some
-                                 (BytesToString
-                                    (fst
-                                       (Vector_split
-                                          (wordToNat (Vector.hd (Guarded_Vector_split 1 n0 b)))
-                                          (n0 - 1 - wordToNat (Vector.hd (Guarded_Vector_split 1 n0 b)))
-                                          (Guarded_Vector_split
-                                             (wordToNat (Vector.hd (Guarded_Vector_split 1 n0 b)))
-                                             (n0 - 1)
-                                             (Vector.tl (Guarded_Vector_split 1 n0 b))))),
-                                  s,
-                                 Ifopt Ifopt fst cd as m Then Some (Nat2pointerT (wordToNat (wtl (wtl (wtl m))))) Else None
-                                 as curPtr
-                                 Then (fst c,
-                                      ((curPtr,
-                                       BytesToString
-                                         (fst
-                                            (Vector_split
-                                               (wordToNat (Vector.hd (Guarded_Vector_split 1 n0 b)))
-                                               (n0 - 1 - wordToNat (Vector.hd (Guarded_Vector_split 1 n0 b)))
-                                               (Guarded_Vector_split
-                                                  (wordToNat (Vector.hd (Guarded_Vector_split 1 n0 b)))
-                                                  (n0 - 1)
-                                                  (Vector.tl (Guarded_Vector_split 1 n0 b)))))) ::
-                                       snd c)%list) Else c)
-                          Else Some
-                                 ((BytesToString
-                                     (fst
-                                        (Vector_split
-                                           (wordToNat (Vector.hd (Guarded_Vector_split 1 n0 b)))
-                                           (n0 - 1 - wordToNat (Vector.hd (Guarded_Vector_split 1 n0 b)))
-                                           (Guarded_Vector_split
-                                              (wordToNat (Vector.hd (Guarded_Vector_split 1 n0 b)))
-                                              (n0 - 1)
-                                              (Vector.tl (Guarded_Vector_split 1 n0 b))))) ++
-                                   String "." d)%string,
-                                  s,
-                                 Ifopt Ifopt fst cd as m Then Some (Nat2pointerT (wordToNat (wtl (wtl (wtl m))))) Else None
-                                 as curPtr
-                                 Then (fst c,
-                                      ((curPtr,
-                                       (BytesToString
-                                          (fst
-                                             (Vector_split
-                                                (wordToNat (Vector.hd (Guarded_Vector_split 1 n0 b)))
-                                                (n0 - 1 - wordToNat (Vector.hd (Guarded_Vector_split 1 n0 b)))
-                                                (Guarded_Vector_split
-                                                  (wordToNat (Vector.hd (Guarded_Vector_split 1 n0 b)))
-                                                  (n0 - 1)
-                                                  (Vector.tl (Guarded_Vector_split 1 n0 b))))) ++
-                                        String "." d)%string) ::
-                                       snd c)%list) Else c))) n3
-               end) n2
-          end
-         else None
-     end
-       | right e => None
+          | right e => None
           end in
     Fix Wf_nat.lt_wf (fun m : nat => Vector.t (word 8) m -> CacheDecode -> option (_ * { n : _ & Vector.t _ n} * CacheDecode)) body sz b cd.
 
-    Lemma byte_align_decode_DomainName {sz}
-      : forall (b : Vector.t (word 8) sz) cd,
+  Lemma byte_align_decode_DomainName {sz}
+    : forall (b : Vector.t (word 8) sz) cd,
       decode_DomainName(build_aligned_ByteString b) cd =
       Ifopt byte_aligned_decode_DomainName b cd as p Then
-    (match p with
-     | (a, b', cd') => Some (a, build_aligned_ByteString (projT2 b'), cd')
-     end)
-    Else None.
-     Proof.
-       unfold If_Opt_Then_Else,decode_DomainName,
-       byte_aligned_decode_DomainName; simpl; intros.
-      eapply optimize_Fix.
-      Focus 3.
-      etransitivity.
-      simpl; intros.
-      erewrite ByteAlign_Decode_w_Measure_le with (m := 1)
-                                                    (dec_a' := Vector.hd)
-                                                    (f := fun cd => addD cd 8);
-        try (intros; unfold decode_word; rewrite aligned_decode_char_eq;
-             reflexivity).
-      Focus 2.
-      intros; assert (n = 0) by omega; subst.
-      revert b1; clear.
-      apply case0; reflexivity.
-      set_refine_evar.
-      etransitivity;
-        [eapply If_sumbool_Then_Else_DecodeBindOpt | ]; simpl.
-      apply optimize_under_match; intros.
-      simpl.
-
-      apply optimize_under_match; intros.
-      simpl.
-      erewrite ByteAlign_Decode_w_Measure_le with (m := 1)
-                                                    (dec_a' := Vector.hd)
-                                                    (f := fun cd => addD cd 8);
-        try (intros; unfold decode_word; rewrite aligned_decode_char_eq;
-             reflexivity).
-      Focus 2.
-      intros; assert (n - 1 = 0) by omega.
-      revert b1; rewrite H3; clear.
-      apply case0; reflexivity.
-      set_refine_evar.
-      simpl.
-      etransitivity;
-        [eapply If_sumbool_Then_Else_DecodeBindOpt | ]; simpl.
-      apply optimize_under_match; intros.
-      simpl.
-      reflexivity.
-      simpl.
-      reflexivity.
-      eapply optimize_under_if_bool.
-      apply optimize_under_match.
-      simpl.
-      intros; higher_order_reflexivity.
-      intros.
-      simpl.
-      2: reflexivity.
-      2: reflexivity.
-      2: simpl.
-      erewrite ByteAlign_Decode_w_Measure_lt with (m := (wordToNat (Vector.hd (Guarded_Vector_split 1 n b0)))) (m_OK := n_eq_0_lt _ a_neq0).
-      Focus 3.
-
-      intros.
-      rewrite decode_string_aligned_ByteString.
-      repeat f_equal.
-  higher_order_reflexivity.
-  higher_order_reflexivity.
-
-  etransitivity;
-    [eapply If_sumbool_Then_Else_DecodeBindOpt | ]; simpl.
-  etransitivity.
-  apply optimize_under_match; intros.
-  subst_refine_evar; simpl; higher_order_reflexivity.
-  subst_refine_evar; apply rewrite_under_LetIn; intros; set_refine_evar.
-  subst_refine_evar; simpl; higher_order_reflexivity.
-  apply optimize_under_match; intros.
-  simpl; higher_order_reflexivity.
-  unfold LetIn.
-  apply optimize_under_if_opt.
-  intros; higher_order_reflexivity.
-  eapply optimize_under_DecodeBindOpt2_both.
-  unfold lt_B_Guarded_Vector_split; simpl.
-  intros; apply H with (b_lt' := rec_aligned_decode_DomainName_OK _ _ a_eq a_neq1).
-  apply H2.
-  intros; eapply H0; eauto.
-  intros; simpl.
-  higher_order_reflexivity.
-  intros; eauto using decode_string_aligned_ByteString_overflow.
-  destruct n; eauto.
-  destruct (wlt_dec (natToWord 8 191) (Vector.hd (Guarded_Vector_split 1 (S n) b0)));
-    eauto.
-  find_if_inside; eauto.
-  simpl.
-  find_if_inside; eauto.
-  destruct n; try omega; simpl; eauto.
-  match goal with
-    |- match ?z with _ => _ end = match match ?z' with _ => _ end with _ => _ end =>
-    replace z' with z by reflexivity; destruct z; eauto
-  end.
-  clear; induction s; simpl; eauto.
-  destruct n; simpl; auto; try omega.
-  match goal with
-    |- match ?z with _ => _ end = match match ?z' with _ => _ end with _ => _ end =>
-    replace z' with z by reflexivity; destruct z; eauto
-  end.
-  match goal with
-    |- match ?z with _ => _ end = match match ?z' with _ => _ end with _ => _ end =>
-    replace z' with z by reflexivity; destruct z; eauto
-  end.
-  find_if_inside; simpl; eauto.
-  match goal with
-    |- match ?z with _ => _ end = match match ?z' with _ => _ end with _ => _ end =>
-    replace z' with z by reflexivity; destruct z; eauto
-  end.
-  match goal with
-    |- (Ifopt ?c as a Then _ Else _) = _ => destruct c as [ ? | ]; simpl; eauto
-  end.
-  match goal with
-    |- DecodeBindOpt2 ?z _ = _ => destruct z as [ [ [? ?] ?] | ]; simpl; eauto
-  end.
-  find_if_inside; simpl; eauto.
-  simpl; intros; apply functional_extensionality; intros.
-  f_equal.
-  simpl; intros; repeat (apply functional_extensionality; intros).
-  destruct (wlt_dec (natToWord 8 191) x1).
-  reflexivity.
-  destruct (wlt_dec x1 (natToWord 8 64)); simpl.
-  destruct (weq x1 (wzero 8)); eauto.
-  match goal with
-    |- DecodeBindOpt2 ?z _ = _ => destruct z as [ [ [? ?] ?] | ]; simpl; eauto
-  end.
-  match goal with
-    |- (Ifopt ?c as a Then _ Else _) = _ => destruct c as [ ? | ]; simpl; eauto
-  end.
-  rewrite H.
-  reflexivity.
-  eauto.
-  simpl; intros; apply functional_extensionality; intros.
-  f_equal.
-  simpl; intros; repeat (apply functional_extensionality; intros).
-  match goal with
-    |- match ?z with _ => _ end = match ?z' with _ => _ end =>
-    replace z' with z by reflexivity; destruct z; eauto
-  end.
-  match goal with
-    |- match ?z with _ => _ end = match ?z' with _ => _ end =>
-    replace z' with z by reflexivity; destruct z; eauto
-  end.
-  find_if_inside; simpl.
-  find_if_inside; simpl; eauto.
-    match goal with
-    |- match ?z with _ => _ end = match ?z' with _ => _ end =>
-    replace z' with z by reflexivity; destruct z; eauto
-  end.
-  match goal with
-    |- (Ifopt ?c as a Then _ Else _) = _ => destruct c as [ ? | ]; simpl; eauto
-  end.
-  rewrite H; reflexivity.
-  eauto.
-  Qed.
-
-  Lemma lift_match_if_ByteAlign
-        {T1}
-        {T2 T3 T4 A : T1 -> Type}
-        {B B' C}
-    : forall (b : bool)
-             (t1 : T1)
-             (t e : option (A t1 * B * C))
-             (b' : forall t1, T2 t1 -> T3 t1 -> T4 t1 -> bool)
-             (t' e' : forall t1, T2 t1 -> T3 t1 -> T4 t1 -> option (A t1 * B' * C))
-             (f : B' -> B)
-             (t2 : T2 t1)
-             (t3 : T3 t1)
-             (t4 : T4 t1),
-      (b = b' t1 t2 t3 t4)
-      -> (t = match t' t1 t2 t3 t4 with
-       | Some (a, b', c) => Some (a, f b', c)
-       | None => None
-           end)
-      -> (e = match e' t1 t2 t3 t4 with
-       | Some (a, b', c) => Some (a, f b', c)
-       | None => None
-              end)
-      -> (if b then t else e) =
-      match (fun t1 t2 t3 t4 => if b' t1 t2 t3 t4 then t' t1 t2 t3 t4 else e' t1 t2 t3 t4) t1 t2 t3 t4 with
-      | Some (a, b', c) => Some (a, f b', c)
-      | None => None
-      end.
+                                                     (match p with
+                                                      | (a, b', cd') => Some (a, build_aligned_ByteString (projT2 b'), cd')
+                                                      end)
+                                                     Else None.
   Proof.
-    intros; destruct b; eauto; rewrite <- H; simpl; eauto.
-  Qed.
+    unfold If_Opt_Then_Else,decode_DomainName,
+    byte_aligned_decode_DomainName; simpl; intros.
+    eapply optimize_Fix.
+    Focus 3.
+    etransitivity.
+    simpl; intros.
+    erewrite ByteAlign_Decode_w_Measure_le with (m := 1)
+                                                  (dec_a' := Vector.hd)
+                                                  (f := fun cd => addD cd 8);
+      try (intros; unfold decode_word; rewrite aligned_decode_char_eq;
+           reflexivity).
+    Focus 2.
+    intros; assert (n = 0) by omega; subst.
+    revert b1; clear.
+    apply case0; reflexivity.
+    set_refine_evar.
+    etransitivity;
+      [eapply If_sumbool_Then_Else_DecodeBindOpt | ]; simpl.
+    apply optimize_under_match; intros.
+    simpl.
 
-  Lemma lift_match_if_sumbool_ByteAlign
-        {T1}
-        {T3 : T1 -> Type}
-        {P : forall t1 (t3 : T3 t1), Prop}
-        {T2 T4 A : T1 -> Type}
-        {B B' C}
-    : forall (t1 : T1)
-             (t3 : T3 t1)
-             (b : forall t1 t3, {P t1 t3} + {~P t1 t3})
-             (t : _ -> option (A t1 * B * C))
-             (e : _ -> option (A t1 * B * C))
-             (b' : forall t1 t3, T2 t1 -> T4 t1 -> {P t1 t3} + {~P t1 t3})
-             (t' : forall t1 t3, T2 t1 -> T4 t1 -> _ -> option (A t1 * B' * C))
-             (e' : forall t1 t3, T2 t1 -> T4 t1 -> _ -> option (A t1 * B' * C))
-             (f : B' -> B)
-             (t2 : T2 t1)
-             (t4 : T4 t1),
-      (b t1 t3 = b' t1 t3 t2 t4)
-      -> (forall e'',
-             t e'' = match t' t1 t3 t2 t4 e'' with
-                    | Some (a, b', c) => Some (a, f b', c)
-                    | None => None
-              end)
-      -> (forall e'',
-             e e'' = match e' t1 t3 t2 t4 e'' with
-                     | Some (a, b', c) => Some (a, f b', c)
-                     | None => None
-                     end)
-      -> (match b t1 t3 with
-            left e'' => t e''
-          | right e'' => e e''
-          end) =
-         match (fun t1 t2 t3 t4 =>
-                  match b' t1 t3 t2 t4 with
-                  | left e'' => t' t1 t3 t2 t4 e''
-                  | right e'' => e' t1 t3 t2 t4 e''
-                  end) t1 t2 t3 t4 with
-      | Some (a, b', c) => Some (a, f b', c)
-      | None => None
-      end.
-  Proof.
-    intros; destruct b; eauto; rewrite <- H; simpl; eauto.
-  Qed.
+    apply optimize_under_match; intros.
+    simpl.
+    erewrite ByteAlign_Decode_w_Measure_le with (m := 1)
+                                                  (dec_a' := Vector.hd)
+                                                  (f := fun cd => addD cd 8);
+      try (intros; unfold decode_word; rewrite aligned_decode_char_eq;
+           reflexivity).
+    Focus 2.
+    intros; assert (n - 1 = 0) by omega.
+    revert b1; rewrite H3; clear.
+    apply case0; reflexivity.
+    set_refine_evar.
+    simpl.
+    etransitivity;
+      [eapply If_sumbool_Then_Else_DecodeBindOpt | ]; simpl.
+    apply optimize_under_match; intros.
+    simpl.
+    reflexivity.
+    simpl.
+    reflexivity.
+    eapply optimize_under_if_bool.
+    apply optimize_under_match.
+    simpl.
+    intros; higher_order_reflexivity.
+    intros.
+    simpl.
+    2: reflexivity.
+    2: reflexivity.
+    2: simpl.
+    erewrite ByteAlign_Decode_w_Measure_lt with (m := (wordToNat (Vector.hd (Guarded_Vector_split 1 n b0)))) (m_OK := n_eq_0_lt _ a_neq0).
+    Focus 3.
 
-    Lemma decode_word_aligned_ByteString_overflow
-        {sz}
-    : forall {sz'}
-             (b : t (word 8) sz')
-             (cd : CacheDecode),
-      lt sz' sz
-      -> decode_word (sz := 8 * sz) (build_aligned_ByteString b) cd = None.
-  Proof.
-  Admitted.
+    intros.
+    rewrite decode_string_aligned_ByteString.
+    repeat f_equal.
+    higher_order_reflexivity.
+    higher_order_reflexivity.
 
-  Lemma build_aligned_ByteString_eq_split'
-    : forall n sz v,
-      (n <= sz)%nat
-      ->
-      build_aligned_ByteString v
-      = build_aligned_ByteString (Guarded_Vector_split n sz v).
-  Proof.
-    intros; eapply ByteString_f_equal; simpl.
-    instantiate (1 := eq_refl _); reflexivity.
-    instantiate (1 := (le_plus_minus_r _ _ H)).
-    generalize (le_plus_minus_r n sz H); clear.
-    revert sz v; induction n; simpl; intros.
-    unfold Guarded_Vector_split.
-    rewrite <- Equality.transport_pp.
-    generalize (eq_trans (minus_n_O sz) e); clear;
-      intro.
-    apply Eqdep_dec.eq_rect_eq_dec; auto with arith.
-    destruct v; simpl in *.
-    omega.
-    unfold Guarded_Vector_split; fold Guarded_Vector_split;
-      simpl.
-    erewrite eq_rect_Vector_cons; eauto.
-    f_equal.
-    apply IHn.
-    Grab Existential Variables.
-    omega.
-  Qed.
-
-  Lemma optimize_Guarded_Decode {sz} {A C} n
-    : forall (a_opt : ByteString -> option (A * ByteString * C))
-             (a_opt' : ByteString -> option (A * ByteString * C)) v,
-      (~ (n <= sz)%nat
-       -> a_opt (build_aligned_ByteString v) = None)
-      -> (le n sz -> a_opt  (build_aligned_ByteString (Guarded_Vector_split n sz v))
-                     = a_opt'
-                         (build_aligned_ByteString (Guarded_Vector_split n sz v)))
-      -> a_opt (build_aligned_ByteString v) =
-         If NPeano.leb n sz Then
-            a_opt' (build_aligned_ByteString (Guarded_Vector_split n sz v))
-            Else None.
-  Proof.
-    intros; destruct (NPeano.leb n sz) eqn: ?.
-    - apply NPeano.leb_le in Heqb.
-      rewrite <- H0.
-      simpl; rewrite <- build_aligned_ByteString_eq_split'; eauto.
+    etransitivity;
+      [eapply If_sumbool_Then_Else_DecodeBindOpt | ]; simpl.
+    etransitivity.
+    apply optimize_under_match; intros.
+    subst_refine_evar; simpl; higher_order_reflexivity.
+    subst_refine_evar; apply rewrite_under_LetIn; intros; set_refine_evar.
+    subst_refine_evar; simpl; higher_order_reflexivity.
+    apply optimize_under_match; intros.
+    simpl; higher_order_reflexivity.
+    unfold LetIn.
+    apply optimize_under_if_opt.
+    intros; higher_order_reflexivity.
+    eapply optimize_under_DecodeBindOpt2_both.
+    unfold lt_B_Guarded_Vector_split; simpl.
+    intros; apply H with (b_lt' := rec_aligned_decode_DomainName_OK _ _ a_eq a_neq1).
+    apply H2.
+    intros; eapply H0; eauto.
+    intros; simpl.
+    higher_order_reflexivity.
+    intros; eauto using decode_string_aligned_ByteString_overflow.
+    destruct n; eauto.
+    destruct (wlt_dec (natToWord 8 191) (Vector.hd (Guarded_Vector_split 1 (S n) b0)));
       eauto.
-    - rewrite H; simpl; eauto.
-      intro.
-      rewrite <- NPeano.leb_le in H1; congruence.
+    find_if_inside; eauto.
+    simpl.
+    find_if_inside; eauto.
+    destruct n; try omega; simpl; eauto.
+    match goal with
+      |- match ?z with _ => _ end = match match ?z' with _ => _ end with _ => _ end =>
+      replace z' with z by reflexivity; destruct z; eauto
+    end.
+    clear; induction s; simpl; eauto.
+    destruct n; simpl; auto; try omega.
+    match goal with
+      |- match ?z with _ => _ end = match match ?z' with _ => _ end with _ => _ end =>
+      replace z' with z by reflexivity; destruct z; eauto
+    end.
+    match goal with
+      |- match ?z with _ => _ end = match match ?z' with _ => _ end with _ => _ end =>
+      replace z' with z by reflexivity; destruct z; eauto
+    end.
+    find_if_inside; simpl; eauto.
+    match goal with
+      |- match ?z with _ => _ end = match match ?z' with _ => _ end with _ => _ end =>
+      replace z' with z by reflexivity; destruct z; eauto
+    end.
+    match goal with
+      |- (Ifopt ?c as a Then _ Else _) = _ => destruct c as [ ? | ]; simpl; eauto
+    end.
+    match goal with
+      |- DecodeBindOpt2 ?z _ = _ => destruct z as [ [ [? ?] ?] | ]; simpl; eauto
+    end.
+    find_if_inside; simpl; eauto.
+    simpl; intros; apply functional_extensionality; intros.
+    f_equal.
+    simpl; intros; repeat (apply functional_extensionality; intros).
+    destruct (wlt_dec (natToWord 8 191) x1).
+    reflexivity.
+    destruct (wlt_dec x1 (natToWord 8 64)); simpl.
+    destruct (weq x1 (wzero 8)); eauto.
+    match goal with
+      |- DecodeBindOpt2 ?z _ = _ => destruct z as [ [ [? ?] ?] | ]; simpl; eauto
+    end.
+    match goal with
+      |- (Ifopt ?c as a Then _ Else _) = _ => destruct c as [ ? | ]; simpl; eauto
+    end.
+    rewrite H.
+    reflexivity.
+    eauto.
+    simpl; intros; apply functional_extensionality; intros.
+    f_equal.
+    simpl; intros; repeat (apply functional_extensionality; intros).
+    match goal with
+      |- match ?z with _ => _ end = match ?z' with _ => _ end =>
+      replace z' with z by reflexivity; destruct z; eauto
+    end.
+    match goal with
+      |- match ?z with _ => _ end = match ?z' with _ => _ end =>
+      replace z' with z by reflexivity; destruct z; eauto
+    end.
+    find_if_inside; simpl.
+    find_if_inside; simpl; eauto.
+    match goal with
+      |- match ?z with _ => _ end = match ?z' with _ => _ end =>
+      replace z' with z by reflexivity; destruct z; eauto
+    end.
+    match goal with
+      |- (Ifopt ?c as a Then _ Else _) = _ => destruct c as [ ? | ]; simpl; eauto
+    end.
+    rewrite H; reflexivity.
+    eauto.
   Qed.
+
 
   Arguments Core.append_word : simpl never.
 
-  Lemma nth_Vector_split {A}
-    : forall {sz} n v idx,
-      (snd (Vector_split (A := A) n sz v))[@idx]
-      = v[@(Fin.R n idx)].
-  Proof.
-    induction n; simpl; intros; eauto.
-    assert (forall A n b, exists a b', b = Vector.cons A a n b')
-      by (clear; intros; pattern n, b; apply caseS; eauto).
-    pose proof (H _ _ v); destruct_ex; subst.
-    simpl.
-    destruct (Vector_split n sz x0) as [? ?] eqn: ?.
-    rewrite <- IHn.
-    rewrite Heqp; reflexivity.
-  Qed.
-
-  Lemma Vector_split_merge {A}
-    : forall sz m n (v : Vector.t A _),
-      snd (Vector_split m _ (snd (Vector_split n (m + sz) v))) =
-      snd (Vector_split (n + m) _ (eq_rect _ _ v _ (plus_assoc _ _ _))).
-  Proof.
-    induction m; intros; simpl.
-    - induction n; simpl.
-      + simpl in *.
-        apply Eqdep_dec.eq_rect_eq_dec; auto with arith.
-      + simpl in v.
-        assert (forall A n b, exists a b', b = Vector.cons A a n b')
-          by (clear; intros; pattern n, b; apply caseS; eauto).
-        pose proof (H _ _ v); destruct_ex; subst.
-        simpl.
-        pose proof (IHn x0).
-        destruct (Vector_split n sz x0) eqn: ?.
-        simpl in *.
-        rewrite H0.
-        erewrite eq_rect_Vector_cons with (H' := (plus_assoc n 0 sz)); eauto; simpl.
-        destruct (Vector_split (n + 0) sz (eq_rect (n + sz) (Vector.t A) x0 (n + 0 + sz) (plus_assoc n 0 sz))); reflexivity.
-    -
-  Admitted.
-
   Arguments Vector_split : simpl never.
 
-  Lemma AlignedDecode4Char {C}
-        {numBytes}
-    : forall (v : Vector.t (word 8) (S (S (S (S numBytes)))))
-             (k : (word 32) -> ByteString -> CacheDecode -> option (C * ByteString * CacheDecode))
-             cd,
-      (`(a, b0, d) <- decode_word
-        (transformerUnit := ByteString_QueueTransformerOpt) (sz := 32) (build_aligned_ByteString v) cd;
-         k a b0 d) =
-      Let n := Core.append_word (Vector.nth v (Fin.FS (Fin.FS (Fin.FS Fin.F1))))
-                                (Core.append_word (Vector.nth v (Fin.FS (Fin.FS Fin.F1)))
-                                                  (Core.append_word (Vector.nth v (Fin.FS Fin.F1)) (Vector.nth v Fin.F1))) in
-        k n (build_aligned_ByteString (snd (Vector_split 4 _ v))) (addD cd 32).
-  Proof.
-    unfold LetIn; intros.
-    unfold decode_word, WordOpt.decode_word.
-    match goal with
-      |- context[Ifopt ?Z as _ Then _ Else _] => replace Z with
-                                                 (let (v', v'') := Vector_split 4 numBytes v in Some (VectorByteToWord v', build_aligned_ByteString v'')) by (symmetry; apply (@aligned_decode_char_eq' _ 3 v))
-    end.
-    Local Transparent Vector_split.
-    unfold Vector_split, If_Opt_Then_Else, DecodeBindOpt2 at 1, If_Opt_Then_Else.
-    f_equal.
-    rewrite !Vector_nth_tl, !Vector_nth_hd.
-    erewrite VectorByteToWord_cons.
-    rewrite <- !Eqdep_dec.eq_rect_eq_dec; eauto using Peano_dec.eq_nat_dec.
-    f_equal.
-    erewrite VectorByteToWord_cons.
-    rewrite <- !Eqdep_dec.eq_rect_eq_dec; eauto using Peano_dec.eq_nat_dec.
-    erewrite VectorByteToWord_cons.
-    rewrite <- !Eqdep_dec.eq_rect_eq_dec; eauto using Peano_dec.eq_nat_dec.
-    erewrite VectorByteToWord_cons.
-    rewrite <- !Eqdep_dec.eq_rect_eq_dec; eauto using Peano_dec.eq_nat_dec.
-    Grab Existential Variables.
-    omega.
-    omega.
-    omega.
-    omega.
-  Qed.
-
-
-
-  Fixpoint align_decode_list {A}
-           (A_decode_align : forall n,
-               Vector.t (word 8) n
-               -> CacheDecode
-               -> option (A * {n : _ & Vector.t _ n}
-                          * CacheDecode))
-           (n : nat)
-           {sz}
-           (v : Vector.t (word 8) sz)
-           (cd : CacheDecode)
-    : option (list A *  {n : _ & Vector.t _ n} * CacheDecode) :=
-    match n with
-    | 0 => Some (@nil _, existT _ _ v, cd)
-    | S s' => `(x, b1, e1) <- A_decode_align sz v cd;
-                `(xs, b2, e2) <- align_decode_list A_decode_align s' (projT2 b1) e1;
-                Some ((x :: xs)%list, b2, e2)
-    end.
-
-  Lemma optimize_align_decode_list
-        {A}
-        (A_decode :
-           ByteString
-           -> CacheDecode
-           -> option (A * ByteString * CacheDecode))
-        (A_decode_align : forall n,
-            Vector.t (word 8) n
-            -> CacheDecode
-            -> option (A * {n : _ & Vector.t _ n}
-                       * CacheDecode))
-        (A_decode_OK :
-           forall n (v : Vector.t _ n) cd,
-             A_decode (build_aligned_ByteString v) cd =
-             Ifopt A_decode_align n v cd as a Then
-                                              Some (fst (fst a), build_aligned_ByteString (projT2 (snd (fst a))), snd a)
-                                              Else
-                                              None)
-    : forall (n : nat)
-             {sz}
-             (v : Vector.t (word 8) sz)
-             (cd : CacheDecode),
-      decode_list A_decode n (build_aligned_ByteString v) cd =
-      Ifopt align_decode_list A_decode_align n v cd as a Then
-                                                         Some (fst (fst a), build_aligned_ByteString (projT2 (snd (fst a))), snd a)
-                                                         Else
-                                                         None.
-  Proof.
-    induction n; simpl; intros; eauto.
-    rewrite A_decode_OK.
-    rewrite (If_Opt_Then_Else_DecodeBindOpt (cache := dns_list_cache)).
-    destruct (A_decode_align sz v cd) as [ [ [? [? ?] ] ?]  | ]; simpl; eauto.
-    rewrite IHn.
-    rewrite (If_Opt_Then_Else_DecodeBindOpt (cache := dns_list_cache)).
-    destruct (align_decode_list A_decode_align n t c)
-      as [ [ [? [? ?] ] ?]  | ]; simpl; eauto.
-  Qed.
-
-  Lemma LetIn_If_Opt_Then_Else {A B C}
-    : forall (a : A)
-             (k : A -> option B)
-             (t : B -> C)
-             (e : C),
-      (Ifopt LetIn a k as b Then t b Else e)
-      = LetIn a (fun a => Ifopt k a as b Then t b Else e).
-  Proof.
-    reflexivity.
-  Qed.
-
-
-  Lemma decode_unused_word_aligned_ByteString_overflow
-        {sz}
-    : forall {sz'}
-             (b : t (word 8) sz')
-             (cd : CacheDecode),
-      lt sz' sz
-      -> decode_unused_word (8 * sz) (build_aligned_ByteString b) cd = None.
-  Proof.
-  Admitted.
-
-
-  Lemma aligned_decode_unused_char_eq
-        {numBytes}
-    : forall (v : Vector.t (word 8) (S numBytes)),
-      WordOpt.decode_unused_word' (transformerUnit := ByteString_QueueTransformerOpt) 8 (build_aligned_ByteString v)
-      = Some ((), build_aligned_ByteString (Vector.tl v)).
-  Proof.
-  Admitted.
-
-  Lemma AlignedDecodeUnusedChars {C}
-        {numBytes numBytes'}
-    : forall (v : Vector.t (word 8) (numBytes' + numBytes))
-             (k : () -> ByteString -> CacheDecode -> option (C * ByteString * CacheDecode))
-             cd,
-      (`(a, b0, d) <- decode_unused_word
-        (transformerUnit := ByteString_QueueTransformerOpt) (8 * numBytes') (build_aligned_ByteString v) cd;
-         k a b0 d) =
-      k () (build_aligned_ByteString (snd (Vector_split numBytes' _ v))) (addD cd (8 * numBytes')).
-  Proof.
-    induction numBytes'; simpl; intros.
-    - Local Transparent Vector_split.
-      unfold Vector_split; simpl.
-      reflexivity.
-      Local Opaque Vector_split.
-    - unfold decode_unused_word.
-      replace (S
-                 (numBytes' +
-                  S
-                    (numBytes' +
-                     S
-                       (numBytes' +
-                        S
-                          (numBytes' +
-                           S (numBytes' + S (numBytes' + S (numBytes' + S (numBytes' + 0))))))))) with (8 + 8 * numBytes') by omega.
-  Admitted.
-
-  Definition align_decode_sumtype
-             {m : nat}
-             {types : t Type m}
-             (decoders :
-                ilist (B := fun T =>
-                              forall n,
-                                Vector.t (word 8) n
-                                -> CacheDecode
-                                -> option (T * {n : _ & Vector.t (word 8) n} * CacheDecode)) types)
-             (idx : Fin.t m)
-             {n : nat}
-             (v : Vector.t (word 8) n)
-             (cd : CacheDecode)
-    := `(a, b', cd') <- ith (decoders) idx n v cd;
-         Some (inj_SumType types idx a, b', cd').
-
-  Lemma align_decode_sumtype_OK'
-        {m : nat}
-        {types : t Type m}
-        (align_decoders :
-           ilist (B := fun T =>
-                         forall n,
-                           Vector.t (word 8) n
-                           -> CacheDecode
-                           -> option (T * {n : _ & Vector.t (word 8) n} * CacheDecode)) types)
-
-        (decoders : ilist (B := fun T => ByteString -> CacheDecode -> option (T * ByteString * CacheDecode)) types)
-        (decoders_OK : forall n v cd idx',
-            ith decoders idx' (build_aligned_ByteString v) cd
-            = Ifopt ith align_decoders idx' n v cd as a Then
-                                                        Some (fst (fst a), build_aligned_ByteString (projT2 (snd (fst a))), snd a)
-                                                        Else
-                                                        None)
-    : forall
-      (idx : Fin.t m)
-      {n : nat}
-      (v : Vector.t (word 8) n)
-      (cd : CacheDecode),
-      decode_SumType types decoders idx (build_aligned_ByteString v) cd
-      =
-      Ifopt align_decode_sumtype align_decoders idx
-            v cd as a Then
-                      Some (fst (fst a), build_aligned_ByteString (projT2 (snd (fst a))), snd a)
-                      Else
-                      None.
-  Proof.
-    intros.
-    unfold decode_SumType, align_decode_sumtype.
-    rewrite decoders_OK.
-    destruct (ith align_decoders idx n v cd) as [ [ [? ?] ?] | ];
-      reflexivity.
-  Qed.
-
-  Corollary align_decode_sumtype_OK
-            {m : nat}
-            {types : t Type m}
-            (align_decoders :
-               ilist (B := fun T =>
-                             forall n,
-                               Vector.t (word 8) n
-                               -> CacheDecode
-                               -> option (T * {n : _ & Vector.t (word 8) n} * CacheDecode)) types)
-
-            (decoders : ilist (B := fun T => ByteString -> CacheDecode -> option (T * ByteString * CacheDecode)) types)
-            (decoders_OK : forall n v cd,
-                Iterate_Ensemble_BoundedIndex
-                  (fun idx' => ith decoders idx' (build_aligned_ByteString v) cd
-                               = Ifopt ith align_decoders idx' n v cd as a Then
-                                                                           Some (fst (fst a), build_aligned_ByteString (projT2 (snd (fst a))), snd a)
-                                                                           Else
-                                                                           None))
-    : forall
-      (idx : Fin.t m)
-      {n : nat}
-      (v : Vector.t (word 8) n)
-      (cd : CacheDecode),
-      decode_SumType types decoders idx (build_aligned_ByteString v) cd
-      =
-      Ifopt align_decode_sumtype align_decoders idx
-            v cd as a Then
-                      Some (fst (fst a), build_aligned_ByteString (projT2 (snd (fst a))), snd a)
-                      Else
-                      None.
-  Proof.
-    intros; eapply align_decode_sumtype_OK'; intros.
-    pose proof (decoders_OK n0 v0 cd0).
-    eapply Iterate_Ensemble_BoundedIndex_equiv in H.
-    apply H.
-  Qed.
   Arguments NPeano.leb : simpl never.
+
+
 
   Definition ByteAligned_packetDecoderImpl n
     : {impl : _ & forall (v : Vector.t _ (12 + n)),
