src/BinEncoders/Env/BinLib/AlignedDecoders.v
@@ -1,0 +1,1013 @@
+Require Import
+        Coq.Strings.String
+        Coq.Arith.Mult
+        Coq.Vectors.Vector.
+
+Require Import
+        Fiat.Examples.DnsServer.SimplePacket
+        Fiat.Common.SumType
+        Fiat.Common.BoundedLookup
+        Fiat.Common.ilist
+        Fiat.Common.DecideableEnsembles
+        Fiat.Computation
+        Fiat.QueryStructure.Specification.Representation.Notations
+        Fiat.QueryStructure.Specification.Representation.Heading
+        Fiat.QueryStructure.Specification.Representation.Tuple
+        Fiat.BinEncoders.Env.BinLib.AlignedByteString
+        Fiat.BinEncoders.Env.BinLib.AlignWord
+        Fiat.BinEncoders.Env.Common.Specs
+        Fiat.BinEncoders.Env.Common.Compose
+        Fiat.BinEncoders.Env.Common.ComposeOpt
+        Fiat.BinEncoders.Env.Automation.Solver
+        Fiat.BinEncoders.Env.Lib2.WordOpt
+        Fiat.BinEncoders.Env.Lib2.NatOpt
+        Fiat.BinEncoders.Env.Lib2.StringOpt
+        Fiat.BinEncoders.Env.Lib2.EnumOpt
+        Fiat.BinEncoders.Env.Lib2.FixListOpt
+        Fiat.BinEncoders.Env.Lib2.SumTypeOpt
+        Fiat.BinEncoders.Env.Lib2.DomainNameOpt
+        Fiat.Common.IterateBoundedIndex
+        Fiat.Common.Tactics.CacheStringConstant.
+
+Require Import
+        Bedrock.Word.
+
+Section AlignedDecoders.
+
+  Context {cache : Cache}.
+  Context {cacheAddNat : CacheAdd cache nat}.
+
+Lemma AlignedDecodeChar {C}
+        {numBytes}
+    : forall (v : Vector.t (word 8) (S numBytes))
+             (k : (word 8) -> ByteString
+                  -> CacheDecode -> option (C * ByteString * CacheDecode))
+             cd,
+      (`(a, b0, d) <- decode_word
+        (transformerUnit := ByteString_QueueTransformerOpt) (sz := 8) (build_aligned_ByteString v) cd;
+         k a b0 d) =
+      LetIn(Vector.nth v Fin.F1)
+           (fun n => k n (build_aligned_ByteString (snd (Vector_split 1 _ v))) (addD cd 8)).
+  Proof.
+    unfold LetIn; intros.
+    unfold decode_word, WordOpt.decode_word.
+    rewrite aligned_decode_char_eq; simpl.
+    f_equal.
+    pattern numBytes, v; apply Vector.caseS; simpl; intros.
+    reflexivity.
+  Qed.
+
+  Lemma AlignedDecode2Char {C}
+        {numBytes}
+    : forall (v : Vector.t (word 8) (S (S numBytes)))
+             (k : (word 16) -> ByteString -> CacheDecode -> option (C * ByteString * CacheDecode))
+             cd,
+      (`(a, b0, d) <- decode_word
+        (transformerUnit := ByteString_QueueTransformerOpt) (sz := 16) (build_aligned_ByteString v) cd;
+         k a b0 d) =
+      Let n := Core.append_word (Vector.nth v (Fin.FS Fin.F1)) (Vector.nth v Fin.F1) in
+        k n (build_aligned_ByteString (snd (Vector_split 2 _ v))) (addD cd 16).
+  Proof.
+    unfold LetIn; intros.
+    unfold decode_word, WordOpt.decode_word.
+    match goal with
+      |- context[Ifopt ?Z as _ Then _ Else _] => replace Z with
+                                                 (let (v', v'') := Vector_split 2 numBytes v in Some (VectorByteToWord v', build_aligned_ByteString v'')) by (symmetry; apply (@aligned_decode_char_eq' _ 1 v))
+    end.
+    unfold Vector_split, If_Opt_Then_Else, DecodeBindOpt2 at 1, If_Opt_Then_Else.
+    f_equal.
+    rewrite !Vector_nth_tl, !Vector_nth_hd.
+    erewrite VectorByteToWord_cons.
+    rewrite <- !Eqdep_dec.eq_rect_eq_dec; eauto using Peano_dec.eq_nat_dec.
+    f_equal.
+    erewrite VectorByteToWord_cons.
+    rewrite <- !Eqdep_dec.eq_rect_eq_dec; eauto using Peano_dec.eq_nat_dec.
+    Grab Existential Variables.
+    omega.
+    omega.
+  Qed.
+
+  Corollary AlignedDecode2Nat {C}
+            {numBytes}
+    : forall (v : Vector.t (word 8) (S (S numBytes)))
+             (k : nat -> ByteString -> CacheDecode -> option (C * ByteString * CacheDecode))
+             cd,
+      (`(a, b0, d) <- decode_nat
+        (transformerUnit := ByteString_QueueTransformerOpt) 16 (build_aligned_ByteString v) cd;
+         k a b0 d) =
+      Let n := wordToNat (Core.append_word (Vector.nth v (Fin.FS Fin.F1)) (Vector.nth v Fin.F1)) in
+        k n (build_aligned_ByteString (snd (Vector_split 2 _ v))) (addD cd 16).
+  Proof.
+    unfold CacheDecode.
+    unfold decode_nat; intros.
+    rewrite DecodeBindOpt2_assoc.
+    unfold DecodeBindOpt2 at 2, If_Opt_Then_Else.
+    rewrite AlignedDecode2Char.
+    reflexivity.
+  Qed.
+
+  Lemma optimize_under_if_opt {A ResultT}
+    : forall (a_opt : option A) (t t' : A -> ResultT) (e e' : ResultT),
+      (forall a, t a = t' a) -> e = e' ->
+      Ifopt a_opt as a Then t a Else e = Ifopt a_opt as a Then t' a Else e'.
+  Proof.
+    intros; subst; eauto.
+    destruct a_opt; eauto.
+  Qed.
+
+  Lemma rewrite_under_LetIn
+        {A B}
+    : forall (a : A) (k k' : A -> B),
+      (forall a, k a = k' a) -> LetIn a k = LetIn a k'.
+  Proof.
+    intros; unfold LetIn; eauto.
+  Qed.
+
+  Fixpoint Guarded_Vector_split
+           (sz n : nat)
+           {struct sz}
+    : Vector.t (word 8) n
+      -> Vector.t (word 8) (sz + (n - sz)) :=
+    match sz, n return
+          Vector.t _ n
+          -> Vector.t (word 8) (sz + (n - sz))
+    with
+    | 0, _ => fun v => (eq_rect _ (Vector.t _) v _ (minus_n_O n))
+    | S n', 0 =>
+      fun v =>
+        Vector.cons _ (wzero _) _ (Guarded_Vector_split n' _ v)
+    | S n', S sz' =>
+      fun v =>
+        Vector.cons _ (Vector.hd v) _ (Guarded_Vector_split n' _ (Vector.tl v))
+    end .
+
+  Lemma le_B_Guarded_Vector_split
+        {n}
+        (b : Vector.t _ n)
+        (m : nat)
+    : {b' : ByteString | le_B b' (build_aligned_ByteString b)}.
+    eexists (build_aligned_ByteString
+               (snd (Vector_split _ _ (Guarded_Vector_split m n b)))).
+    abstract (unfold build_aligned_ByteString, le_B; simpl; omega).
+  Defined.
+
+
+  Lemma build_aligned_ByteString_eq_split
+    : forall m n b H0,
+      (m <= n)%nat
+      -> build_aligned_ByteString b =
+         (build_aligned_ByteString (eq_rect (m + (n - m)) (t (word 8)) (Guarded_Vector_split m n b) n H0)).
+  Proof.
+    intros.
+    intros; eapply ByteString_f_equal; simpl.
+    instantiate (1 := eq_refl _); reflexivity.
+    instantiate (1 := eq_refl _).
+    simpl.
+    revert n b H0 H; induction m; simpl.
+    intros ? ?; generalize (minus_n_O n).
+    intros; rewrite <- Equality.transport_pp.
+    apply Eqdep_dec.eq_rect_eq_dec; auto with arith.
+    intros.
+    inversion H; subst.
+    - revert b H0 IHm; clear.
+      intro; pattern m, b; apply Vector.caseS; simpl; intros.
+      assert ((n + (n - n)) = n) by omega.
+      rewrite eq_rect_Vector_cons with (H' := H).
+      f_equal.
+      erewrite <- IHm; eauto.
+    - revert b H0 IHm H1; clear.
+      intro; pattern m0, b; apply Vector.caseS; simpl; intros.
+      assert ((m + (n - m)) = n) by omega.
+      erewrite eq_rect_Vector_cons with (H' := H).
+      f_equal.
+      erewrite <- IHm; eauto.
+      omega.
+  Qed.
+
+  Lemma ByteAlign_Decode_w_Measure_le {A}
+    : forall (dec_a : ByteString -> CacheDecode -> option (A * ByteString * CacheDecode))
+             (n m : nat)
+             (dec_a' : Vector.t (word 8) (m + (n - m)) -> A)
+             (cd : CacheDecode)
+             (f : CacheDecode -> CacheDecode)
+             (b : Vector.t (word 8) n)
+             decode_a_le
+             (dec_fail : ~ (m <= n)%nat
+                         -> forall b cd, dec_a (build_aligned_ByteString (numBytes := n) b) cd = None),
+      (forall b cd, dec_a (build_aligned_ByteString b) cd =
+                    Some (dec_a' b, build_aligned_ByteString (snd (Vector_split m (n - m) b)), f cd))
+      -> Decode_w_Measure_le dec_a (build_aligned_ByteString b) cd decode_a_le =
+         match Compare_dec.le_dec m n with
+         | left e => (Let a := dec_a' (Guarded_Vector_split m n b) in
+                          Some (a, le_B_Guarded_Vector_split b m, f cd))
+         | right _ => None
+         end.
+  Proof.
+    intros.
+    destruct (Compare_dec.le_dec m n).
+    assert (m + (n - m) = n) by omega.
+    assert (forall b, Decode_w_Measure_le dec_a (build_aligned_ByteString b) cd decode_a_le
+                      = Decode_w_Measure_le dec_a (build_aligned_ByteString ( eq_rect _ _ (Guarded_Vector_split m n b) _ H0)) cd decode_a_le).
+    { revert l; clear; intros.
+      destruct (Decode_w_Measure_le dec_a (build_aligned_ByteString b) cd decode_a_le)
+        as [ [ [? [? ?] ] ?] | ] eqn: ?.
+      apply Decode_w_Measure_le_eq' in Heqo.
+      simpl in Heqo.
+      destruct (Decode_w_Measure_le dec_a
+                                    (build_aligned_ByteString (eq_rect (m + (n - m)) (t (word 8)) (Guarded_Vector_split m n b) n H0)) cd decode_a_le) as [ [ [? [? ?] ] ?] | ] eqn: ?.
+      apply Decode_w_Measure_le_eq' in Heqo0.
+      simpl in *.
+      rewrite <- build_aligned_ByteString_eq_split in Heqo0 by eauto.
+      rewrite Heqo0 in Heqo.
+      injection Heqo; intros.
+      rewrite H, H2;
+        repeat f_equal.
+      revert l0 l1. rewrite H1; intros; f_equal.
+      f_equal; apply Core.le_uniqueness_proof.
+      apply ByteString_id.
+      eapply Decode_w_Measure_le_eq'' in Heqo0.
+      rewrite <- build_aligned_ByteString_eq_split in Heqo0 by eauto.
+      rewrite Heqo0 in Heqo.
+      discriminate.
+      apply ByteString_id.
+      erewrite build_aligned_ByteString_eq_split in Heqo by eauto.
+      rewrite Heqo; reflexivity.
+    }
+    rewrite H1.
+    match goal with
+      |- ?a = _ => destruct a as [ [ [? ?] ? ] | ] eqn: ?
+    end.
+    eapply Decode_w_Measure_le_eq' in Heqo.
+    assert (dec_a (build_aligned_ByteString (Guarded_Vector_split m n b)) cd
+            = Some (a, projT1 s, c)).
+    { destruct s; simpl in *.
+      rewrite <- Heqo.
+      unfold build_aligned_ByteString; repeat f_equal; simpl.
+      eapply ByteString_f_equal; simpl.
+      instantiate (1 := eq_refl _); reflexivity.
+      instantiate (1 := sym_eq H0).
+      clear H1.
+      destruct H0; reflexivity.
+    }
+    rewrite H in H2; injection H2; intros.
+    rewrite H3, H5; unfold LetIn; simpl.
+    repeat f_equal.
+    destruct s; simpl in *.
+    unfold le_B_Guarded_Vector_split; simpl.
+    clear H1; revert l0.
+    rewrite <- H4; intros.
+    f_equal; apply Core.le_uniqueness_proof.
+    apply ByteString_id.
+    apply Decode_w_Measure_le_eq'' in Heqo.
+    pose proof (H (Guarded_Vector_split m n b) cd).
+    assert (Some (dec_a' (Guarded_Vector_split m n b),
+                  build_aligned_ByteString (snd (Vector_split m (n - m) (Guarded_Vector_split m n b))),
+                  f cd) = None).
+    { rewrite <- Heqo.
+      rewrite <- H.
+      repeat f_equal.
+      eapply ByteString_f_equal; simpl.
+      instantiate (1 := eq_refl _); reflexivity.
+      instantiate (1 := sym_eq H0).
+      clear H1.
+      destruct H0; reflexivity.
+    }
+    discriminate.
+    eapply dec_fail in n0; simpl.
+    eapply Specs.Decode_w_Measure_le_eq' in n0.
+    apply n0.
+  Qed.
+
+  Lemma lt_B_Guarded_Vector_split
+        {n}
+        (b : Vector.t _ n)
+        (m : nat)
+        (m_OK : lt 0 m)
+        (_ : ~ lt n m)
+    : {b' : ByteString | lt_B b' (build_aligned_ByteString b)}.
+    eexists (build_aligned_ByteString
+               (snd (Vector_split _ _ (Guarded_Vector_split m n b)))).
+    abstract (unfold build_aligned_ByteString, lt_B; simpl; omega).
+  Defined.
+
+  Lemma decode_string_aligned_ByteString
+        {sz sz'}
+    : forall (b : t (word 8) (sz + sz'))
+             (cd : CacheDecode),
+      FixStringOpt.decode_string sz (build_aligned_ByteString b) cd =
+      Some (BytesToString (fst (Vector_split sz sz' b)),
+            build_aligned_ByteString (snd (Vector_split sz sz' b)),
+            addD cd (8 * sz)).
+  Proof.
+    induction sz; intros.
+    - simpl; repeat f_equal.
+      destruct cd as [ [? | ] ? ]; unfold addD; simpl.
+      pose proof (wordToNat_bound w); find_if_inside; try omega.
+      rewrite plus_comm; simpl; rewrite natToWord_wordToNat; reflexivity.
+      reflexivity.
+    - simpl.
+      assert (forall A n b, exists a b', b = Vector.cons A a n b')
+        by (clear; intros; pattern n, b; apply caseS; eauto).
+      destruct (H _ _ b) as [? [? ?] ]; subst; simpl.
+      unfold AsciiOpt.decode_ascii.
+      rewrite DecodeBindOpt2_assoc; simpl.
+      etransitivity.
+      rewrite AlignedDecodeChar; simpl.
+      rewrite IHsz. higher_order_reflexivity.
+      simpl.
+      destruct (Vector_split sz sz' x0); simpl.
+      unfold LetIn.
+      rewrite addD_addD_plus;
+        repeat f_equal.
+      omega.
+  Qed.
+
+  Lemma decode_string_aligned_ByteString_overflow
+        {sz}
+    : forall {sz'}
+             (b : t (word 8) sz')
+             (cd : CacheDecode),
+      lt sz' sz
+      -> FixStringOpt.decode_string sz (build_aligned_ByteString b) cd = None.
+  Proof.
+    induction sz; intros.
+    - omega.
+    - simpl.
+      assert (forall A n b, exists a b', b = Vector.cons A a n b')
+        by (clear; intros; pattern n, b; apply caseS; eauto).
+      destruct sz'.
+      + reflexivity.
+      + destruct (H0 _ _ b) as [? [? ?] ]; subst; simpl.
+        unfold AsciiOpt.decode_ascii.
+        rewrite DecodeBindOpt2_assoc; simpl.
+        etransitivity.
+        rewrite AlignedDecodeChar; simpl.
+        rewrite IHsz. higher_order_reflexivity.
+        omega.
+        reflexivity.
+  Qed.
+
+  Lemma ByteAlign_Decode_w_Measure_lt {A}
+    : forall (dec_a : nat -> ByteString -> CacheDecode -> option (A * ByteString * CacheDecode))
+             (n m : nat)
+             (dec_a' : forall m n, Vector.t (word 8) (m + n) -> A)
+             (cd : CacheDecode)
+             (f : nat -> CacheDecode -> CacheDecode)
+             (b : Vector.t (word 8) n)
+             (m_OK : lt 0 m)
+             decode_a_le
+             (dec_fail : (lt n m)%nat
+                         -> forall b cd, dec_a m (build_aligned_ByteString (numBytes := n) b) cd = None),
+      (forall n m b cd, dec_a m (build_aligned_ByteString b) cd =
+                        Some (dec_a' _ _ b, build_aligned_ByteString (snd (Vector_split m n b)), f m cd))
+      -> Decode_w_Measure_lt (dec_a m) (build_aligned_ByteString b) cd decode_a_le =
+         match Compare_dec.lt_dec n m with
+         | left _ => None
+         | right n' => (Let a := dec_a' _ _ (Guarded_Vector_split m n b) in
+                            Some (a, lt_B_Guarded_Vector_split b m m_OK n' , f m cd))
+         end.
+  Proof.
+    intros.
+    destruct (Compare_dec.lt_dec m n);
+      destruct (Compare_dec.lt_dec n m); try omega.
+    - assert (m + (n - m) = n) by omega.
+      assert (forall b, Decode_w_Measure_lt (dec_a m) (build_aligned_ByteString b) cd decode_a_le
+                        = Decode_w_Measure_lt (dec_a m)(build_aligned_ByteString ( eq_rect _ _ (Guarded_Vector_split m n b) _ H0)) cd decode_a_le).
+      { revert l; clear; intros.
+        destruct (Decode_w_Measure_lt (dec_a m) (build_aligned_ByteString b) cd decode_a_le)
+          as [ [ [? [? ?] ] ?] | ] eqn: ?.
+        apply Decode_w_Measure_lt_eq' in Heqo.
+        simpl in Heqo.
+        destruct (Decode_w_Measure_lt (dec_a m)
+                                      (build_aligned_ByteString (eq_rect _ (t (word 8)) (Guarded_Vector_split m n b) n H0)) cd decode_a_le) as [ [ [? [? ?] ] ?] | ] eqn: ?.
+        apply Decode_w_Measure_lt_eq' in Heqo0.
+        unfold proj1_sig in Heqo0.
+        rewrite <- build_aligned_ByteString_eq_split in Heqo0.
+        rewrite Heqo0 in Heqo.
+        injection Heqo; intros.
+        rewrite H, H2;
+          repeat f_equal.
+        revert l1 l0. rewrite H1; intros; f_equal.
+        f_equal; apply Core.le_uniqueness_proof.
+        omega.
+        apply ByteString_id.
+        eapply Decode_w_Measure_lt_eq'' in Heqo0.
+        rewrite <- build_aligned_ByteString_eq_split in Heqo0 by omega.
+        rewrite Heqo0 in Heqo.
+        discriminate.
+        apply ByteString_id.
+        erewrite (build_aligned_ByteString_eq_split m n) in Heqo by omega.
+        rewrite Heqo; reflexivity.
+      }
+      rewrite H1.
+      match goal with
+        |- ?a = _ => destruct a as [ [ [? ?] ? ] | ] eqn: ?
+      end.
+      eapply Decode_w_Measure_lt_eq' in Heqo.
+      assert (dec_a m (build_aligned_ByteString (Guarded_Vector_split m n b)) cd
+              = Some (a, projT1 s, c)).
+      { destruct s; simpl in *.
+        rewrite <- Heqo.
+        unfold build_aligned_ByteString; repeat f_equal; simpl.
+        eapply ByteString_f_equal; simpl.
+        instantiate (1 := eq_refl _); reflexivity.
+        instantiate (1 := sym_eq H0).
+        clear H1.
+        destruct H0; reflexivity.
+      }
+      rewrite H in H2; injection H2; intros.
+      rewrite H3, H5; unfold LetIn; simpl.
+      repeat f_equal.
+      destruct s; simpl in *.
+      unfold lt_B_Guarded_Vector_split; simpl.
+      clear H1; revert l0.
+      rewrite <- H4; intros.
+      f_equal. apply Core.le_uniqueness_proof.
+      apply ByteString_id.
+      apply Decode_w_Measure_lt_eq'' in Heqo.
+      pose proof (H _ _ (Guarded_Vector_split m n b) cd).
+      assert (Some (dec_a' _ _ (Guarded_Vector_split m n b),
+                    build_aligned_ByteString (snd (Vector_split m (n - m) (Guarded_Vector_split m n b))),
+                    f m cd) = None).
+      { rewrite <- Heqo.
+        rewrite <- H.
+        repeat f_equal.
+        eapply ByteString_f_equal; simpl.
+        instantiate (1 := eq_refl _); reflexivity.
+        instantiate (1 := sym_eq H0).
+        clear H1.
+        destruct H0; reflexivity.
+      }
+      discriminate.
+    - eapply dec_fail in l; simpl.
+      eapply Specs.Decode_w_Measure_lt_eq' in l.
+      apply l.
+    - assert (m = n) by omega; subst.
+      assert (n + (n - n) = n) by omega.
+      assert (forall b, Decode_w_Measure_lt (dec_a n) (build_aligned_ByteString b) cd decode_a_le
+                        = Decode_w_Measure_lt (dec_a n)(build_aligned_ByteString ( eq_rect _ _ (Guarded_Vector_split n n b) _ H0)) cd decode_a_le).
+      { clear; intros.
+        destruct (Decode_w_Measure_lt (dec_a n) (build_aligned_ByteString b) cd decode_a_le)
+          as [ [ [? [? ?] ] ?] | ] eqn: ?.
+        apply Decode_w_Measure_lt_eq' in Heqo.
+        simpl in Heqo.
+        destruct (Decode_w_Measure_lt (dec_a n)
+                                      (build_aligned_ByteString (eq_rect _ (t (word 8)) (Guarded_Vector_split n n b) n H0)) cd decode_a_le) as [ [ [? [? ?] ] ?] | ] eqn: ?.
+        apply Decode_w_Measure_lt_eq' in Heqo0.
+        unfold proj1_sig in Heqo0.
+        rewrite <- build_aligned_ByteString_eq_split in Heqo0.
+        rewrite Heqo0 in Heqo.
+        injection Heqo; intros.
+        rewrite H, H2;
+          repeat f_equal.
+        revert l l0. rewrite H1; intros; f_equal.
+        f_equal; apply Core.le_uniqueness_proof.
+        omega.
+        apply ByteString_id.
+        eapply Decode_w_Measure_lt_eq'' in Heqo0.
+        rewrite <- build_aligned_ByteString_eq_split in Heqo0 by omega.
+        rewrite Heqo0 in Heqo.
+        discriminate.
+        apply ByteString_id.
+        erewrite (build_aligned_ByteString_eq_split n n) in Heqo by omega.
+        rewrite Heqo; reflexivity.
+      }
+      rewrite H1.
+      match goal with
+        |- ?a = _ => destruct a as [ [ [? ?] ? ] | ] eqn: ?
+      end.
+      eapply Decode_w_Measure_lt_eq' in Heqo.
+      assert (dec_a n (build_aligned_ByteString (Guarded_Vector_split n n b)) cd
+              = Some (a, projT1 s, c)).
+      { destruct s; simpl in *.
+        rewrite <- Heqo.
+        unfold build_aligned_ByteString; repeat f_equal; simpl.
+        eapply ByteString_f_equal; simpl.
+        instantiate (1 := eq_refl _); reflexivity.
+        instantiate (1 := sym_eq H0).
+        clear H1.
+        destruct H0; reflexivity.
+      }
+      rewrite H in H2; injection H2; intros.
+      rewrite H3, H5; unfold LetIn; simpl.
+      repeat f_equal.
+      destruct s; simpl in *.
+      unfold lt_B_Guarded_Vector_split; simpl.
+      clear H1; revert l.
+      rewrite <- H4; intros.
+      f_equal. apply Core.le_uniqueness_proof.
+      apply ByteString_id.
+      apply Decode_w_Measure_lt_eq'' in Heqo.
+      pose proof (H _ _ (Guarded_Vector_split n n b) cd).
+      assert (Some (dec_a' _ _ (Guarded_Vector_split n n b),
+                    build_aligned_ByteString (snd (Vector_split n (n - n) (Guarded_Vector_split n n b))),
+                    f n cd) = None).
+      { rewrite <- Heqo.
+        rewrite <- H.
+        repeat f_equal.
+        eapply ByteString_f_equal; simpl.
+        instantiate (1 := eq_refl _); reflexivity.
+        instantiate (1 := sym_eq H0).
+        clear H1.
+        destruct H0; reflexivity.
+      }
+      discriminate.
+  Qed.
+
+  Lemma optimize_under_match {A B} {P}
+    : forall (a a' : A) (f : {P a a'} + {~P a a'}) (t t' : _ -> B)
+             (e e' : _ -> B),
+      (forall (a a' : A) (a_eq : _), t a_eq = t' a_eq)
+      -> (forall (a a' : A) (a_neq : _), e a_neq = e' a_neq)
+      -> match f with
+         | left e => t e
+         | right n => e n
+         end =
+         match f with
+         | left e => t' e
+         | right n => e' n
+         end.
+  Proof.
+    destruct f; simpl; intros; eauto.
+  Qed.
+
+  Lemma optimize_Fix {A}
+    : forall
+      (body : forall x : ByteString,
+          (forall y : ByteString,
+              lt_B y x -> (fun _ : ByteString => CacheDecode -> option (A * ByteString * CacheDecode)) y) ->
+          (fun _ : ByteString => CacheDecode -> option (A * ByteString * CacheDecode)) x)
+      (body' : forall x : nat,
+          (forall y : nat,
+              (lt y x)%nat ->
+              (fun m : nat =>
+                 t (word 8) m -> CacheDecode ->
+                 option (A * {n : _ & Vector.t _ n} * CacheDecode)) y) ->
+          t (word 8) x -> CacheDecode -> option (A * {n : _ & Vector.t _ n} * CacheDecode) )
+      n (b : Vector.t _ n) (cd : CacheDecode)
+      (body_Proper :
+         forall (x0 : ByteString)
+                (f g : forall y : ByteString, lt_B y x0 -> CacheDecode -> option (A * ByteString * CacheDecode)),
+           (forall (y : ByteString) (p : lt_B y x0), f y p = g y p) -> body x0 f = body x0 g)
+      (body'_Proper :
+         forall (x0 : nat)
+                (f
+                   g : forall y : nat,
+                    (lt y x0)%nat -> t (word 8) y -> CacheDecode -> option (A * {n0 : nat & t Core.char n0} * CacheDecode)),
+           (forall (y : nat) (p : (lt y x0)%nat), f y p = g y p) -> body' x0 f = body' x0 g)
+    ,
+      (forall n (b : Vector.t (word 8) n)
+              (rec : forall x : ByteString,
+                  lt_B x (build_aligned_ByteString b) -> CacheDecode -> option (A * ByteString * CacheDecode))
+              (rec' : forall x : nat,
+                  (lt x n)%nat -> t Core.char x -> CacheDecode ->
+                  option (A * {n : _ & Vector.t _ n} * CacheDecode))
+              cd,
+          (forall m cd b a b' cd' b_lt b_lt' ,
+              rec' m b_lt' b cd = Some (a, b', cd')
+              -> rec (build_aligned_ByteString b) b_lt cd = Some (a, build_aligned_ByteString (projT2 b'), cd'))
+          -> (forall m cd b b_lt b_lt' ,
+                 rec' m b_lt' b cd = None
+                 -> rec (build_aligned_ByteString b) b_lt cd = None)
+          -> body (build_aligned_ByteString b) rec cd
+             = match (body' n rec' b cd) with
+               | Some (a, b', cd') => Some (a, build_aligned_ByteString (projT2 b'), cd')
+               | None => None
+               end)
+      -> Fix well_founded_lt_b (fun _ : ByteString => CacheDecode -> option (A * ByteString * CacheDecode)) body (build_aligned_ByteString b) cd =
+         match Fix Wf_nat.lt_wf (fun m : nat => Vector.t (word 8) m -> CacheDecode -> option (A * { n : _ & Vector.t _ n} * CacheDecode)) body' n b cd with
+         | Some (a, b', cd') => Some (a, build_aligned_ByteString (projT2 b'), cd')
+         | None => None
+         end.
+  Proof.
+    intros.
+    revert cd b; pattern n.
+    eapply (well_founded_ind Wf_nat.lt_wf); intros.
+    rewrite Init.Wf.Fix_eq, Init.Wf.Fix_eq.
+    apply H; intros.
+    erewrite H0, H1; eauto.
+    rewrite H0, H1; eauto.
+    eauto.
+    eauto.
+  Qed.
+
+  Lemma lift_match_if_ByteAlign
+        {T1}
+        {T2 T3 T4 A : T1 -> Type}
+        {B B' C}
+    : forall (b : bool)
+             (t1 : T1)
+             (t e : option (A t1 * B * C))
+             (b' : forall t1, T2 t1 -> T3 t1 -> T4 t1 -> bool)
+             (t' e' : forall t1, T2 t1 -> T3 t1 -> T4 t1 -> option (A t1 * B' * C))
+             (f : B' -> B)
+             (t2 : T2 t1)
+             (t3 : T3 t1)
+             (t4 : T4 t1),
+      (b = b' t1 t2 t3 t4)
+      -> (t = match t' t1 t2 t3 t4 with
+              | Some (a, b', c) => Some (a, f b', c)
+              | None => None
+              end)
+      -> (e = match e' t1 t2 t3 t4 with
+              | Some (a, b', c) => Some (a, f b', c)
+              | None => None
+              end)
+      -> (if b then t else e) =
+         match (fun t1 t2 t3 t4 => if b' t1 t2 t3 t4 then t' t1 t2 t3 t4 else e' t1 t2 t3 t4) t1 t2 t3 t4 with
+         | Some (a, b', c) => Some (a, f b', c)
+         | None => None
+         end.
+  Proof.
+    intros; destruct b; eauto; rewrite <- H; simpl; eauto.
+  Qed.
+
+  Lemma lift_match_if_sumbool_ByteAlign
+        {T1}
+        {T3 : T1 -> Type}
+        {P : forall t1 (t3 : T3 t1), Prop}
+        {T2 T4 A : T1 -> Type}
+        {B B' C}
+    : forall (t1 : T1)
+             (t3 : T3 t1)
+             (b : forall t1 t3, {P t1 t3} + {~P t1 t3})
+             (t : _ -> option (A t1 * B * C))
+             (e : _ -> option (A t1 * B * C))
+             (b' : forall t1 t3, T2 t1 -> T4 t1 -> {P t1 t3} + {~P t1 t3})
+             (t' : forall t1 t3, T2 t1 -> T4 t1 -> _ -> option (A t1 * B' * C))
+             (e' : forall t1 t3, T2 t1 -> T4 t1 -> _ -> option (A t1 * B' * C))
+             (f : B' -> B)
+             (t2 : T2 t1)
+             (t4 : T4 t1),
+      (b t1 t3 = b' t1 t3 t2 t4)
+      -> (forall e'',
+             t e'' = match t' t1 t3 t2 t4 e'' with
+                     | Some (a, b', c) => Some (a, f b', c)
+                     | None => None
+                     end)
+      -> (forall e'',
+             e e'' = match e' t1 t3 t2 t4 e'' with
+                     | Some (a, b', c) => Some (a, f b', c)
+                     | None => None
+                     end)
+      -> (match b t1 t3 with
+            left e'' => t e''
+          | right e'' => e e''
+          end) =
+         match (fun t1 t2 t3 t4 =>
+                  match b' t1 t3 t2 t4 with
+                  | left e'' => t' t1 t3 t2 t4 e''
+                  | right e'' => e' t1 t3 t2 t4 e''
+                  end) t1 t2 t3 t4 with
+         | Some (a, b', c) => Some (a, f b', c)
+         | None => None
+         end.
+  Proof.
+    intros; destruct b; eauto; rewrite <- H; simpl; eauto.
+  Qed.
+
+  Lemma decode_word_aligned_ByteString_overflow
+        {sz}
+    : forall {sz'}
+             (b : t (word 8) sz')
+             (cd : CacheDecode),
+      lt sz' sz
+      -> decode_word (sz := 8 * sz) (build_aligned_ByteString b) cd = None.
+  Proof.
+  Admitted.
+
+  Lemma build_aligned_ByteString_eq_split'
+    : forall n sz v,
+      (n <= sz)%nat
+      ->
+      build_aligned_ByteString v
+      = build_aligned_ByteString (Guarded_Vector_split n sz v).
+  Proof.
+    intros; eapply ByteString_f_equal; simpl.
+    instantiate (1 := eq_refl _); reflexivity.
+    instantiate (1 := (le_plus_minus_r _ _ H)).
+    generalize (le_plus_minus_r n sz H); clear.
+    revert sz v; induction n; simpl; intros.
+    unfold Guarded_Vector_split.
+    rewrite <- Equality.transport_pp.
+    generalize (eq_trans (minus_n_O sz) e); clear;
+      intro.
+    apply Eqdep_dec.eq_rect_eq_dec; auto with arith.
+    destruct v; simpl in *.
+    omega.
+    unfold Guarded_Vector_split; fold Guarded_Vector_split;
+      simpl.
+    erewrite eq_rect_Vector_cons; eauto.
+    f_equal.
+    apply IHn.
+    Grab Existential Variables.
+    omega.
+  Qed.
+
+  Lemma optimize_Guarded_Decode {sz} {A C} n
+    : forall (a_opt : ByteString -> option (A * ByteString * C))
+             (a_opt' : ByteString -> option (A * ByteString * C)) v,
+      (~ (n <= sz)%nat
+       -> a_opt (build_aligned_ByteString v) = None)
+      -> (le n sz -> a_opt  (build_aligned_ByteString (Guarded_Vector_split n sz v))
+                     = a_opt'
+                         (build_aligned_ByteString (Guarded_Vector_split n sz v)))
+      -> a_opt (build_aligned_ByteString v) =
+         If NPeano.leb n sz Then
+            a_opt' (build_aligned_ByteString (Guarded_Vector_split n sz v))
+            Else None.
+  Proof.
+    intros; destruct (NPeano.leb n sz) eqn: ?.
+    - apply NPeano.leb_le in Heqb.
+      rewrite <- H0.
+      simpl; rewrite <- build_aligned_ByteString_eq_split'; eauto.
+      eauto.
+    - rewrite H; simpl; eauto.
+      intro.
+      rewrite <- NPeano.leb_le in H1; congruence.
+  Qed.
+
+  Lemma AlignedDecode4Char {C}
+        {numBytes}
+    : forall (v : Vector.t (word 8) (S (S (S (S numBytes)))))
+             (k : (word 32) -> ByteString -> CacheDecode -> option (C * ByteString * CacheDecode))
+             cd,
+      (`(a, b0, d) <- decode_word
+        (transformerUnit := ByteString_QueueTransformerOpt) (sz := 32) (build_aligned_ByteString v) cd;
+         k a b0 d) =
+      Let n := Core.append_word (Vector.nth v (Fin.FS (Fin.FS (Fin.FS Fin.F1))))
+                                (Core.append_word (Vector.nth v (Fin.FS (Fin.FS Fin.F1)))
+                                                  (Core.append_word (Vector.nth v (Fin.FS Fin.F1)) (Vector.nth v Fin.F1))) in
+        k n (build_aligned_ByteString (snd (Vector_split 4 _ v))) (addD cd 32).
+  Proof.
+    unfold LetIn; intros.
+    unfold decode_word, WordOpt.decode_word.
+    match goal with
+      |- context[Ifopt ?Z as _ Then _ Else _] => replace Z with
+                                                 (let (v', v'') := Vector_split 4 numBytes v in Some (VectorByteToWord v', build_aligned_ByteString v'')) by (symmetry; apply (@aligned_decode_char_eq' _ 3 v))
+    end.
+    Local Transparent Vector_split.
+    unfold Vector_split, If_Opt_Then_Else, DecodeBindOpt2 at 1, If_Opt_Then_Else.
+    f_equal.
+    rewrite !Vector_nth_tl, !Vector_nth_hd.
+    erewrite VectorByteToWord_cons.
+    rewrite <- !Eqdep_dec.eq_rect_eq_dec; eauto using Peano_dec.eq_nat_dec.
+    f_equal.
+    erewrite VectorByteToWord_cons.
+    rewrite <- !Eqdep_dec.eq_rect_eq_dec; eauto using Peano_dec.eq_nat_dec.
+    erewrite VectorByteToWord_cons.
+    rewrite <- !Eqdep_dec.eq_rect_eq_dec; eauto using Peano_dec.eq_nat_dec.
+    erewrite VectorByteToWord_cons.
+    rewrite <- !Eqdep_dec.eq_rect_eq_dec; eauto using Peano_dec.eq_nat_dec.
+    Grab Existential Variables.
+    omega.
+    omega.
+    omega.
+    omega.
+  Qed.
+
+
+
+  Fixpoint align_decode_list {A}
+           (A_decode_align : forall n,
+               Vector.t (word 8) n
+               -> CacheDecode
+               -> option (A * {n : _ & Vector.t _ n}
+                          * CacheDecode))
+           (n : nat)
+           {sz}
+           (v : Vector.t (word 8) sz)
+           (cd : CacheDecode)
+    : option (list A *  {n : _ & Vector.t _ n} * CacheDecode) :=
+    match n with
+    | 0 => Some (@nil _, existT _ _ v, cd)
+    | S s' => `(x, b1, e1) <- A_decode_align sz v cd;
+                `(xs, b2, e2) <- align_decode_list A_decode_align s' (projT2 b1) e1;
+                Some ((x :: xs)%list, b2, e2)
+    end.
+
+  Lemma optimize_align_decode_list
+        {A}
+        (A_decode :
+           ByteString
+           -> CacheDecode
+           -> option (A * ByteString * CacheDecode))
+        (A_decode_align : forall n,
+            Vector.t (word 8) n
+            -> CacheDecode
+            -> option (A * {n : _ & Vector.t _ n}
+                       * CacheDecode))
+        (A_decode_OK :
+           forall n (v : Vector.t _ n) cd,
+             A_decode (build_aligned_ByteString v) cd =
+             Ifopt A_decode_align n v cd as a Then
+                                              Some (fst (fst a), build_aligned_ByteString (projT2 (snd (fst a))), snd a)
+                                              Else
+                                              None)
+    : forall (n : nat)
+             {sz}
+             (v : Vector.t (word 8) sz)
+             (cd : CacheDecode),
+      decode_list A_decode n (build_aligned_ByteString v) cd =
+      Ifopt align_decode_list A_decode_align n v cd as a Then
+                                                         Some (fst (fst a), build_aligned_ByteString (projT2 (snd (fst a))), snd a)
+                                                         Else
+                                                         None.
+  Proof.
+    induction n; simpl; intros; eauto.
+    rewrite A_decode_OK.
+    rewrite (If_Opt_Then_Else_DecodeBindOpt (cache := dns_list_cache)).
+    destruct (A_decode_align sz v cd) as [ [ [? [? ?] ] ?]  | ]; simpl; eauto.
+    rewrite IHn.
+    rewrite (If_Opt_Then_Else_DecodeBindOpt (cache := dns_list_cache)).
+    destruct (align_decode_list A_decode_align n t c)
+      as [ [ [? [? ?] ] ?]  | ]; simpl; eauto.
+  Qed.
+
+  Lemma LetIn_If_Opt_Then_Else {A B C}
+    : forall (a : A)
+             (k : A -> option B)
+             (t : B -> C)
+             (e : C),
+      (Ifopt LetIn a k as b Then t b Else e)
+      = LetIn a (fun a => Ifopt k a as b Then t b Else e).
+  Proof.
+    reflexivity.
+  Qed.
+
+
+  Lemma decode_unused_word_aligned_ByteString_overflow
+        {sz}
+    : forall {sz'}
+             (b : t (word 8) sz')
+             (cd : CacheDecode),
+      lt sz' sz
+      -> decode_unused_word (8 * sz) (build_aligned_ByteString b) cd = None.
+  Proof.
+  Admitted.
+
+
+  Lemma aligned_decode_unused_char_eq
+        {numBytes}
+    : forall (v : Vector.t (word 8) (S numBytes)),
+      WordOpt.decode_unused_word' (transformerUnit := ByteString_QueueTransformerOpt) 8 (build_aligned_ByteString v)
+      = Some ((), build_aligned_ByteString (Vector.tl v)).
+  Proof.
+  Admitted.
+
+  Lemma AlignedDecodeUnusedChars {C}
+        {numBytes numBytes'}
+    : forall (v : Vector.t (word 8) (numBytes' + numBytes))
+             (k : () -> ByteString -> CacheDecode -> option (C * ByteString * CacheDecode))
+             cd,
+      (`(a, b0, d) <- decode_unused_word
+        (transformerUnit := ByteString_QueueTransformerOpt) (8 * numBytes') (build_aligned_ByteString v) cd;
+         k a b0 d) =
+      k () (build_aligned_ByteString (snd (Vector_split numBytes' _ v))) (addD cd (8 * numBytes')).
+  Proof.
+    induction numBytes'; simpl; intros.
+    - Local Transparent Vector_split.
+      unfold Vector_split; simpl.
+      reflexivity.
+      Local Opaque Vector_split.
+    - unfold decode_unused_word.
+      replace (S
+                 (numBytes' +
+                  S
+                    (numBytes' +
+                     S
+                       (numBytes' +
+                        S
+                          (numBytes' +
+                           S (numBytes' + S (numBytes' + S (numBytes' + S (numBytes' + 0))))))))) with (8 + 8 * numBytes') by omega.
+  Admitted.
+
+  Definition align_decode_sumtype
+             {m : nat}
+             {types : t Type m}
+             (decoders :
+                ilist (B := fun T =>
+                              forall n,
+                                Vector.t (word 8) n
+                                -> CacheDecode
+                                -> option (T * {n : _ & Vector.t (word 8) n} * CacheDecode)) types)
+             (idx : Fin.t m)
+             {n : nat}
+             (v : Vector.t (word 8) n)
+             (cd : CacheDecode)
+    := `(a, b', cd') <- ith (decoders) idx n v cd;
+         Some (inj_SumType types idx a, b', cd').
+
+  Lemma align_decode_sumtype_OK'
+        {m : nat}
+        {types : t Type m}
+        (align_decoders :
+           ilist (B := fun T =>
+                         forall n,
+                           Vector.t (word 8) n
+                           -> CacheDecode
+                           -> option (T * {n : _ & Vector.t (word 8) n} * CacheDecode)) types)
+
+        (decoders : ilist (B := fun T => ByteString -> CacheDecode -> option (T * ByteString * CacheDecode)) types)
+        (decoders_OK : forall n v cd idx',
+            ith decoders idx' (build_aligned_ByteString v) cd
+            = Ifopt ith align_decoders idx' n v cd as a Then
+                                                        Some (fst (fst a), build_aligned_ByteString (projT2 (snd (fst a))), snd a)
+                                                        Else
+                                                        None)
+    : forall
+      (idx : Fin.t m)
+      {n : nat}
+      (v : Vector.t (word 8) n)
+      (cd : CacheDecode),
+      decode_SumType types decoders idx (build_aligned_ByteString v) cd
+      =
+      Ifopt align_decode_sumtype align_decoders idx
+            v cd as a Then
+                      Some (fst (fst a), build_aligned_ByteString (projT2 (snd (fst a))), snd a)
+                      Else
+                      None.
+  Proof.
+    intros.
+    unfold decode_SumType, align_decode_sumtype.
+    rewrite decoders_OK.
+    destruct (ith align_decoders idx n v cd) as [ [ [? ?] ?] | ];
+      reflexivity.
+  Qed.
+
+  Corollary align_decode_sumtype_OK
+            {m : nat}
+            {types : t Type m}
+            (align_decoders :
+               ilist (B := fun T =>
+                             forall n,
+                               Vector.t (word 8) n
+                               -> CacheDecode
+                               -> option (T * {n : _ & Vector.t (word 8) n} * CacheDecode)) types)
+
+            (decoders : ilist (B := fun T => ByteString -> CacheDecode -> option (T * ByteString * CacheDecode)) types)
+            (decoders_OK : forall n v cd,
+                Iterate_Ensemble_BoundedIndex
+                  (fun idx' => ith decoders idx' (build_aligned_ByteString v) cd
+                               = Ifopt ith align_decoders idx' n v cd as a Then
+                                                                           Some (fst (fst a), build_aligned_ByteString (projT2 (snd (fst a))), snd a)
+                                                                           Else
+                                                                           None))
+    : forall
+      (idx : Fin.t m)
+      {n : nat}
+      (v : Vector.t (word 8) n)
+      (cd : CacheDecode),
+      decode_SumType types decoders idx (build_aligned_ByteString v) cd
+      =
+      Ifopt align_decode_sumtype align_decoders idx
+            v cd as a Then
+                      Some (fst (fst a), build_aligned_ByteString (projT2 (snd (fst a))), snd a)
+                      Else
+                      None.
+  Proof.
+    intros; eapply align_decode_sumtype_OK'; intros.
+    pose proof (decoders_OK n0 v0 cd0).
+    eapply Iterate_Ensemble_BoundedIndex_equiv in H.
+    apply H.
+  Qed.
+
+  Lemma nth_Vector_split {A}
+    : forall {sz} n v idx,
+      (snd (Vector_split (A := A) n sz v))[@idx]
+      = v[@(Fin.R n idx)].
+  Proof.
+    induction n; simpl; intros; eauto.
+    assert (forall A n b, exists a b', b = Vector.cons A a n b')
+      by (clear; intros; pattern n, b; apply caseS; eauto).
+    pose proof (H _ _ v); destruct_ex; subst.
+    simpl.
+    destruct (Vector_split n sz x0) as [? ?] eqn: ?.
+    rewrite <- IHn.
+    rewrite Heqp; reflexivity.
+  Qed.
+
+  Lemma Vector_split_merge {A}
+    : forall sz m n (v : Vector.t A _),
+      snd (Vector_split m _ (snd (Vector_split n (m + sz) v))) =
+      snd (Vector_split (n + m) _ (eq_rect _ _ v _ (plus_assoc _ _ _))).
+  Proof.
+    induction m; intros; simpl.
+    - induction n; simpl.
+      + simpl in *.
+        apply Eqdep_dec.eq_rect_eq_dec; auto with arith.
+      + simpl in v.
+        assert (forall A n b, exists a b', b = Vector.cons A a n b')
+          by (clear; intros; pattern n, b; apply caseS; eauto).
+        pose proof (H _ _ v); destruct_ex; subst.
+        simpl.
+        pose proof (IHn x0).
+        destruct (Vector_split n sz x0) eqn: ?.
+        simpl in *.
+        rewrite H0.
+        erewrite eq_rect_Vector_cons with (H' := (plus_assoc n 0 sz)); eauto; simpl.
+        destruct (Vector_split (n + 0) sz (eq_rect (n + sz) (Vector.t A) x0 (n + 0 + sz) (plus_assoc n 0 sz))); reflexivity.
+    -
+  Admitted.
+
+End
